<section xml:id="s_FTC">
    <title>Fundamental theorem of calculus</title>
    <p>
        We have now met the two main operations in calculus:
        <md>
            <mrow>\text{Derivative: } f \amp \mapsto f'</mrow>
            <mrow>\text{Integral: } f \amp \mapsto \int_a^b f(x)\, dx </mrow>
        </md>.
        The <xref ref="th_FTC" text="custom">fundamental theorem of calculus (FTC)</xref> how these two operations (derivative and integral) interact. The theorem has two parts (<xref ref="th_FTC_I" text="title"/> and <xref ref="th_FTC_II" text="title"/>). We will focus on FTC II in this section, and FTC I in the next. 
    </p>
    <theorem xml:id="th_FTC">
        <title>Fundamental theorem of calculus</title>
        <statement>
            <p>
                Let <m>f</m> be continuous on <m>I=[a,b]</m>. 
                <ol>
                    <li xml:id="th_FTC_I">
                        <title>FTC I</title>
                        <p>
                            The function <m>F</m> defined on <m>I</m> as 
                            <men xml:id="eq_intregal_function">
                                F(x)=\int_a^x f(t)\, dt
                            </men>
                        is differentiable on <m>I</m> and satisfies 
                        <men xml:id="eq_FTC_I">
                            F'(x)=\frac{d}{dx}\int_a^x f(t)\, dt = f(x)
                        </men>
                        for all <m>x\in I</m>.
                        </p>
                    </li>
                    <li xml:id="th_FTC_II">
                        <title>FTC II</title>
                        <p>
                            If <m>F</m> is an antiderivative of <m>f</m> on <m>I</m>, then 
                            <men xml:id="eq_FTC_II">
                                \int_a^b f(x)\, dx=F(b)-F(a)
                            </men>.
                        </p>
                    </li>
                </ol>
            </p>
        </statement>
        <proof>
            <title>Proof of <xref ref="th_FTC_II" text="title"/></title>
            <p>
                Since <m>f</m> is continuous on <m>[a,b]</m> it is integrable, and thus we can compute its integral as a limit of Riemann sums corresponding to any sequence of pointed partitions <m>P_n</m> satisfying <m>\lVert P_n\rVert\to\infty</m>. The strategy of the proof that follows is to pick these pointed partitions in a <em>very particular way</em> that ensures the value of of the integral we seek.  
            </p>
            <p>
                Let <m>F</m> be an antiderivative of <m>f</m> on <m>I=[a,b]</m>. Since <m>f</m> is continuous on <m>I</m>, we see that <m>F</m> is differentiable on <m>I</m> and its derivative <m>F'=f</m> is continuous. The <em>mean value theorem</em> thus applies to <m>F</m>: given any interval <m>[c,d]</m> on which <m>F'</m> is defined and continuous, there is an element <m>x^*\in[c,d]</m> such that 
                <me>F'(x^*)=\frac{F(d)-F(c)}{d-c}</me>. 
                We use this fact to produce a sequence of pointed partitions  <m>P_n</m> of a very particular sort. Namely for each <m>n</m>, we divide <m>[a,b]</m> into <m>n</m> equal subintervals of length <m>\Delta x=(b-a)/n</m>, and for each subinterval <m>I_k=[x_{k_1},x_k]</m> we choose our sample input <m>c_k</m> to be a point where we have 
                <me>
                    F'(c_k)=\frac{F(x_k)-F(x_{k-1})}{x_k-x_{k-1}}=\frac{F(x_k)-F(x_{k-1})}{\Delta x}
                </me>.
                As discussed above, such a <m>c_k</m> is guaranteed to exist by the mean value theorem.
                Since <m>F'=f</m> by assumption, these sample points satisfy 
                <men xml:id="eq_FTC_II_proof">
                    f(c_k)=\frac{F(x_k)-F(x_{k-1})}{\Delta x}
                </men>.   
                 Note that we have <m>\lVert P_n\rVert=\Delta x=(b-a)/n</m>, and thus <m>\lVert P_n\rVert\to\infty</m>. It follows that if <m>S_n</m> is the Riemann sum corresponding to the pointed partition <m>P_n</m>, then 
                 <me>
                    \int_a^b f(x)\, dx=\lim_{n\to\infty}S_n
                 </me>.
                 We now compute <m>S_n</m> for any fixed <m>n</m>:
                 <md>
                    <mrow>S_n \amp =\sum_{k=1}^nf(c_k)\Delta x</mrow>
                    <mrow> \amp = \sum_{k=1}\left( \frac{F(x_k)-F(x_{k-1})}{\Delta x}\right)\Delta x \amp <xref ref="eq_FTC_II_proof"/></mrow>
                    <mrow> \amp =\sum_{k=1}^n F(x_k)-F(x_{k-1}) </mrow>
                    <mrow> \amp =(\cancel{F(x_1)}-F(x_0))+(\cancel{F(x_2)}-\cancel{F(x_1)}+\cdots (F(x_n)-\cancel{F(x_{n-1}})</mrow>
                    <mrow> \amp =F(x_n)-F(x_0)</mrow>
                    <mrow> \amp =F(b)-F(a)</mrow>
                 </md>.
                 We've shown that <m>S_n=F(b)-F(a)</m> for all <m>n</m>. It follows that 
                 <me>
                    \int_a^b f(x)\, dx=\lim_{n\to\infty}S_n=\lim_{n\to\infty}F(b)-F(a)=F(b)-F(a)
                 </me>,
                 as desired. 
            </p>
        </proof>
    </theorem>
    <p>
        As mentioned above, we will focus here on <xref ref="th_FTC_II" text="title"/>. It main computational import of this theorem is that it allows us to compute definite integrals <em>indirectly</em>, by first finding an antiderivative of the integrand, and then using <xref ref="eq_FTC_II"/>. 
    </p>
    <algorithm xml:id="proc_integral_antiderivative">
        <title>Computing integrals with antiderivatives</title>
        <statement>
            <p>
                Let <m>f</m> be an integrable function on <m>I=[a,b]</m>. To compute <m>\int_a^b f\, dx</m> using antiderivatives, proceed as follows:
                <ol>
                    <li>
                        <p>
                            Find an antiderivative <m>F</m> of <m>f</m> on I. 
                        </p>
                    </li>
                    <li>
                        <p>
                            Use <xref ref="th_FTC_II" text="title"/> to conclude 
                            <me>
                                \int_a^bf(x)\, dx=F(b)-F(a)
                            </me>. 
                        </p>
                    </li>
                </ol> 
            </p>
        </statement>
    </algorithm>
    <p>
        <xref ref="th_FTC_II" text="title"/> allows us to reduce a definite integral computation essentially to finding an antiderivative of the integrand: <ie/>, we integrate basically by <q>computing derivatives in reverse</q>. The Augustus De Morgan quote below captures this quite poetically.
    </p>
    <principle xml:id="mantra_integration_differentiation">
        <title>Integration is differentiation in reverse</title>
        
        <statement>
            <p>
                <q>Common integration is only the memory of differentiation</q>--Augustus De Morgan. 
            </p>
        </statement>
    </principle>
    <p>
        Henceforth our integral computations will involve many expressions of the form <m>F(b)-F(a)</m>, which we call a <em>difference evaluation</em>. It will be useful to have some compact notation for this. 
    </p>
    <definition xml:id="d_difference_evaluation">
        <title>Difference evaluation notation</title>
        <statement>
            <p>
                Let <m>g</m> be a function containing <m>a</m> and <m>b</m> in its domain. We define <m>g]_a^b</m> to be the <term>difference evaluation</term> expression 
                <me>
                    g(x)\Bigr\vert_a^b=g(b)-g(a)
                </me>.                
            </p>
        </statement>
    </definition>
    <remark>
        <title>Difference evaluation notation</title>
        <p>
            <ol>
                <li>
                    <p>
                        It is easy to see that the following difference evaluation identities hold:
                        <md>
                            <mrow>(f(x)+g(x))\Bigr\vert_a^b \amp = f(x)\Bigr\vert_a^b+g(x)\Bigr\vert_a^b </mrow>
                            <mrow>cf(x)\Bigr\vert_a^b \amp = c\left(f(x)\Bigr\vert_a^b\right)</mrow>
                        </md>
                    </p>
                </li>
                <li>
                    <p>
                        Observe that <xref ref="eq_FTC_II"/> can be expressed using our new notation as 
                        <me>
                            \int_a^b f(x)\, dx= F(x)\Bigr\vert_a^b
                        </me>.                        
                    </p>
                </li>
            </ol>
        </p>
        
    </remark>
    <example xml:id="eg_FTCII">
        <title>Computing integrals with antiderivatives</title> 
        <statement>
            <p>
                Use the <xref ref="th_FTC_II" text="title"/> to compute the following definite integrals.
                <ol>
                  <li>
                    <p>
                      <m>\displaystyle\int_a^b 1-x^3\, dx</m>
                    </p>
                  </li>
                  <li>
                    <p>
                      <m>\displaystyle\int_0^{10} \frac{1}{\sqrt{2t+1}}\, dt</m>
                    </p>
                  </li>
                  <li>
                    <p>
                      <m>\displaystyle\int_{3\pi/4}^{\pi}\sec^2 u\, du</m>.
                    </p>
                  </li>
                </ol>
              </p>
        </statement>
        <solution>
            <p>
                Following <xref ref="proc_integral_antiderivative"/>, for each integral we provide an antiderivative <m>F</m> of the integrand <m>f</m> and then compute the integral as a difference evaluation using <xref ref="th_FTC_II" text="title"/>. The integrands in question are familiar and/or simple enough that we do not justify the fact that <m>F</m> is indeed an antiderivative. 
            <ol>
                <li>
                    <p>
                        The function <m>F(x)=x-\frac{1}{4}x^4</m> is an antiderivative of <m>f(x)=1-x^3</m>. It follows from <xref ref="th_FTC_II" text="title"/> that 
                        <md>
                            <mrow>\int_a^b 1-x^3\, dx\amp = F(b)-F(a)</mrow>
                            <mrow> \amp = b-\frac{1}{4}b^4-(a-\frac{1}{4}a^4</mrow>
                            <mrow> \amp =(b-a)-\frac{1}{4}(b^4-a^4)</mrow>
                        </md>.
                    </p>
                </li>
                <li>
                    <p>
                        The function <m>F(x)=\sqrt{2t+1}</m> is an antiderivative of <m>f(t)=1/\sqrt{2t+1}</m>. It follows from <xref ref="th_FTC_II" text="title"/> that 
                        <md>
                            <mrow>\int_0^10\frac{1}{\sqrt{2t+1}}\, dt \amp = F(10)-F(0)</mrow>
                            <mrow>\amp = \sqrt{21}-\sqrt{1} </mrow>
                            <mrow> \amp =\sqrt{21}-1</mrow>
                        </md>.
                    </p>
                </li>
                <li>
                    <p>
                        The function <m>F(x)=\tan u</m> is an antiderivative of <m>f(u)=\sec^2 u</m>. It follows from <xref ref="th_FTC_II" text="title"/> that 
                        <md>
                            <mrow>\int_{3\pi/4}^\pi \sec^2 u\, du  \amp = F(\pi)-F(3\pi/4)</mrow>
                            <mrow> \amp =\tan \pi -\tan(3\pi/4)</mrow>
                            <mrow> \amp =0-(-1)</mrow>
                            <mrow> \amp = 1</mrow>
                        </md>.
                    </p>
                </li>
            </ol>
            </p>
        </solution>
    </example>
    <example xml:id="eg_FTCII_area">
        <title>Signed area using FTC II</title>
        <statement>
            <p>
                Let <m>f(x)=\sin(x/3)</m>,
                and let <m>\mathcal{C}</m> be the graph of <m>f</m>.
                For each region <m>\mathcal{R}</m> compute the area of
                <m>\mathcal{R}</m> and the signed area of <m>\mathcal{R}</m>.
                Include a diagram of <m>\mathcal{C}</m> and <m>\mathcal{R}</m>.
                Make sure your answer is consistent with your graph.
                If your answer happens to be 0, use the diagram to explain why.
                <ol>
                  <li>
                    <p>
                      <m>\mathcal{R}</m> is the region between
                      <m>\mathcal{C}</m> and the <m>x</m>-axis,
                      from <m>x=-\pi</m> to <m>x=\pi</m>.
                    </p>
                  </li>
                  <li>
                    <p>
                      <m>\mathcal{R}</m> is the region between
                      <m>\mathcal{C}</m> and the <m>x</m>-axis,
                      from <m>x=-\pi</m> to <m>x=\pi/2</m>.
                    </p>
                  </li>
                  <li>
                    <p>
                      <m>\mathcal{R}</m> is the region between
                      <m>\mathcal{C}</m> and the <m>x</m>-axis,
                      from <m>x=0</m> to <m>x=6\pi</m>.
                    </p>
                  </li>
                </ol>
              </p>
        </statement>
        <solution>
            <p>
                In each of the cases below we use our definitions of the <xref ref="d_area" text="custom">area</xref> and <xref ref="d_signedarea" text="custom">signed area</xref> of the region <m>\mathcal{R}</m> associated to <m>f</m>:
                <md>
                    <mrow>\operatorname{sgn\, area}\mathcal{R} \amp = \int_a^b f(x)\, dx</mrow>
                    <mrow>\operatorname{area}\mathcal{R} \amp = \int_a^b\abs{f(x)}\, dx</mrow>
                </md>.
            Throughout we will use the fact that <m>F(x)=-3\cos(x/3)</m> is an antiderivative of <m>f(x)=\sin(x/3)</m>. 
            <ol>
                <li>
                    <p>
                        We have
                        <md>
                            <mrow>\operatorname{sgn\, area}\mathcal{R} \amp = \int_{-\pi}^{\pi}f(x)\, dx</mrow>
                            <mrow> \amp =F(\pi)-F(-\pi)</mrow>
                            <mrow> \amp =-3(\cos(\pi/3)-\cos(-\pi/3))=0</mrow>
                            <mrow>\operatorname{area}\mathcal{R} \amp = \int_a^b\abs{f(x)}\, dx</mrow>
                            <mrow> \amp = \int_{-\pi}^0\abs{f}\, dx+\int_0^{\pi}\abs{f} \amp (<xref ref="th_interval_partition" text="title"/>)</mrow>
                            <mrow> \amp = \int_{-\pi}^0-f(x)\, dx+\int_0^\pi f(x)\, dx \amp (\text{def. of } \abs{f})</mrow>
                            <mrow> \amp = -\int_{-\pi}^0f(x)\, dx+\int_0^\pi f(x)\, dx</mrow>
                            <mrow> \amp =-(F(0)-F(-\pi))+(F(\pi)-F(0))</mrow>
                            <mrow> \amp = -(-3\cos 0-(-3)\cos(-\pi/3))+(-3\cos(\pi/3)-(-3)\cos 0)</mrow>
                            <mrow> \amp = 6-3=3</mrow>
                        </md>. 
                        Below you find a diagram of <m>\mathcal{R}</m> described as a union <m>\mathcal{R}=\mathcal{R}_1\cup \mathcal{R}_2</m>. By the symmetry in the diagram it should come as no surprise that 
                        <me>
                            \operatorname{sgn\, area}\mathcal{R}=-\operatorname{area}\mathcal{R}_1+\mathcal{R}_2=0
                        </me>.
                    </p>
                    <image source="images/sgn_area_a.png" width="75%">
                        <description>Part (a) region</description>
                    </image>
                </li>
                <li>
                    <p>
                        The reasoning and computations here are very similar. We get 
                        <md>
                            <mrow>\operatorname{sgn\, area}\mathcal{R} \amp =\int_{-\pi}^{\pi/2}f(x)\, dx    </mrow>
                            <mrow> \amp = \frac{3}{2}-\frac{3\sqrt{3}}{2}</mrow>
                            <mrow>\operatorname{area}\mathcal{R} \amp \int_{-\pi}^{\pi/2}\abs{f}\, dx </mrow>
                            <mrow> \amp = \frac{9}{2}-\frac{3\sqrt{3}}{2}</mrow>
                        </md>.
                    </p>
                </li>
                <li>
                    <p>
                        Again, the reasoning and computations are similar. We get 
                        <md>
                            <mrow>\operatorname{sgn\, area}\mathcal{R} \amp =\int_{0}^{6\pi}f(x)\, dx    </mrow>
                            <mrow> \amp =0 </mrow>
                            <mrow>\operatorname{area}\mathcal{R} \amp \int_{0}^{6\pi}\abs{f}\, dx </mrow>
                            <mrow> \amp = \int_0^{3\pi}f(x)\, dx-\int_{3\pi}^{6\pi}f(x)\, dx</mrow>
                            <mrow> \amp = 6+6=12</mrow>
                        </md>.
                        Both the fact that signed area here is zero and the symmetry appearing in the two terms  of the area computation arises from the fact that <m>\mathcal{R}=\mathcal{R}_1\cup \mathcal{R}_2</m> is a union of two symmetric regions.
                    </p>
                    <image source="images/sgn_area_c.png" width="75%">
                        <description>Signed area over entire period</description>
                    </image>
                </li>
            </ol>
            </p>
        </solution>
    </example>
    <theorem xml:id="th_FTC_II_rate">
        <title>FTC II: rate of change version</title>
        <statement>
            <p>
               Suppose <m>Q=g(x)</m> is a differentiable function on <m>[a,b]</m>. Since <m>g</m> is an antiderivative of <m>g'</m> on <m>I</m>, by <xref ref="th_FTC_II" text="title"/> we have  
               <me>
                \int_a^bg'(x)\, dx = g(b)-g(a)=\Delta Q
               </me>.
               Interpreting <m>g'</m> as a rate of change, we see that integrating the <em>rate of change</em> of a quantity <m>Q</m> from <m>x=a</m> to <m>x=b</m> yields the <em>net change</em> of <m>Q</m> as we vary <m>x</m> from <m>x=a</m> to <m>x=b</m>.
            </p>
        </statement>
    </theorem>
    <example>
        <title>Leaking water tank revisited</title>
        <p>
            Recall the set up from <xref ref="eg_water_tank"/>, where we determined that at time <m>t</m>, the amount of water <m>A=f(t)</m> has rate of change <m>f'(t)=-1/\sqrt{2t+1}</m>.
        </p>
        <p> 
            According to <xref ref="th_FTC_II_rate"/>, for any <m>t=b</m> the integral  
            <me>
                \int_0^b f'(t)\, dt=\int_0^b-1/\sqrt{2t+1}\, dt
            </me>
            computes the <em>net change</em> in the amount of water in the tank between time <m>t=0</m> and <m>t=b</m> minutes: <ie/>, it computes <m>\Delta A=f(b)-f(0)</m>. We can use <xref ref="th_FTC_II" text="title"/> to compute this integral. The function <m>F(x)=-\sqrt{2t+1}</m> is an antiderivative of <m>-1/\sqrt{2t+1}</m> and thus 
            <me>
                \int_0^b -1/\sqrt{2t+1}\, dt=F(b)-F(0)=1-\sqrt{2b+1}
            </me>. 
            This tells us that <m>\Delta A=1-\sqrt{2b+1}</m> at any time <m>b</m>. Since <m>\Delta A=f(b)-f(0)</m>, we conclude that <m>f(b)-f(0)=1-\sqrt{2b+1}</m>, or equivalently, <m>f(b)=f(0)+1-\sqrt{2b+1}=101-\sqrt{2t+1}</m> for all <m>b</m>.  (Here we use the fact that <m>f(0)=100</m>.) We have just given another derivation of the formula 
            <me>
                f(t)=101-\sqrt{2t+1}
            </me>
            for the function <m>A=f(t)</m>.   
        </p>
        
    </example>
</section>