<?xml version="1.0" encoding="UTF-8"?>

<section xml:id="s_inverse" xmlns:xi="http://www.w3.org/2001/XInclude">
    <title>Inverse functions</title>
<definition xml:id="d_one-to-one">
    <title>One-to-one function</title>
    <statement>
        <p>
          A function <m>f</m> is <term>one-to-one</term> on its domain <m>D</m> if <m>f(x_1)\ne f(x_2)</m> for all
          <m>x_1, x_2\in D</m> with <m>x_1\ne x_2</m>.
          We express this with logical notation as
          <me>
            x_1\ne x_2\implies f(x_1)\ne f(x_2)
          </me>,
          or equivalently, using the contrapositive,
          <me>
            f(x_1)=f(x_2)\implies x_1=x_2
          </me>.
        </p>
      </statement>
</definition>

<definition xml:id="d_invertible">
  <title>Inverse function</title>
  
  <statement>
      <p>
        Suppose <m>f</m> is one-to-one on its domain <m>D</m>,
        and let <m>R</m> be the range of <m>f</m>.
        The <term>inverse function</term> of <m>f</m>
        is the function <m>f^{-1}</m> with domain <m>R</m> defined by the following rule: for any <m>b\in R</m>, we define <m>f^{-1}(b)</m> to be the unique <m>a\in D</m> such that <m>f(a)=b</m>. In other words, <m>f^{-1}</m> is the unique function with domain <m>R</m> satisfying 
        <men xml:id="eq_inverse">
          f^{-1}(b)=a \iff b=f(a)
        </men>
        for all elements <m>b</m> in <m>R</m>. 
      </p>
    </statement>
</definition>

<theorem xml:id="th_horizontal_line">
  <title>Horizontal line test</title>
  <statement>
    <p>
      Let <m>f</m> be a function with domain <m>D</m>,
      and let <m>\mathcal{C}</m> be the graph of <m>f</m>.
      The function <m>f</m> is one-to-one on <m>D</m> if and only if for all <m>c\in\R</m> the horizontal line <m>y=c</m> intersects <m>\mathcal{C}</m> in
      <em>at most</em> one point.
    </p>
  </statement>
</theorem>

<definition xml:id="d_monotonic">
    <title>Monotonic</title>
    <statement>
        <p>
          Let <m>f</m> be a a real-valued function with domain <m>D</m>.
          <ul>
            <li>
              <p>
                The function <m>f</m> is <term>increasing</term> on <m>D</m>
                if <m>f(x_1)\lt f(x_2)</m> for all
                <m>x_1, x_2\in D</m> with <m>x_1\lt x_2</m>.
                Using logical notation:
                <me>
                  x_1\lt x_2\implies f(x_1)\lt f(x_2)
                </me>.
              </p>
            </li>
            <li>
              <p>
                The function <m>f</m> is <term>decreasing</term> on <m>D</m>
                if <m>f(x_1)>f(x_2)</m> for all
                <m>x_1, x_2\in D</m> with <m>x_1\lt x_2</m>.
                Using logical notation:
                <me>
                  x_1\lt x_2\implies f(x_1)>f(x_2)
                </me>.
              </p>
            </li>
            <li>
              <p>
                The function <m>f</m> is <term>monotonic</term> on <m>D</m>
                if <m>f</m> is increasing on <m>X</m> or <m>f</m> is decreasing on <m>X</m>.
              </p>
            </li>
          </ul>
        </p>
      </statement>
</definition>



<theorem xml:id="th_monotonic">
  <title>Monotonic functions are one-to-one</title>
  <statement>
    <p>
      If <m>f</m> is monotonic on its domain <m>D</m>, then <m>f</m> is one-to-one on <m>D</m> and hence has an inverse function.
    </p>
  </statement>
</theorem>

<example xml:id="eg_inverse">
  <title>Computing inverse</title>
  <statement>
    <p>
      Let <m>f(x)=x^2+1</m>.
      <ol>
        <li>
          <p>
            Show that <m>f</m> is not one-to-one on <m>D=(-\infty, \infty)</m>.
          </p>
        </li>
        <li>
          <p>
            Show that <m>f</m> is one-to-one on <m>D=(-\infty, 0]</m> and compute an inverse of <m>f</m> with respect to this domain.
          </p>
        </li>
      </ol>
    </p>
  </statement>
  <solution>
    <p>
            Using simple properties of quadratic functions, we know that <m>f</m> is decreasing on <m>(-\infty, 0]</m> and increasing on <m>[0,\infty)</m>. It follows that <m>f</m> is one-to-one on either of those smaller subintervals. Since <m>f(-2)=f(2)=5</m>, and more generally <m>f(-x)=f(x)</m> for all <m>x\in \R
            </m>, we see that <m>f</m> is not one-to-one on <m>\R=(-\infty,\infty)</m>. 
    </p>
    <p>
      Now restrict to the domain <m>D=(-\infty, 0]</m>. By definition, the domain of <m>f^{-1}</m> is the range of <m>y</m>, which is easily seen to be <m>R=[1,\infty)</m>. Given <m>y\in [1,\infty)</m>, to compute <m>f^{-1}(y)</m> we must find the unique <m>x\in D=(-\infty,0]</m> satisfying <m>f(x)=y</m>. Solving this equation for <m>x</m>, we see that  
      <md>
        <mrow>f(x)=y \amp \iff x^2+1=y</mrow>
        <mrow> \amp \iff x^2=y-1 </mrow>
        <mrow> \amp \iff x=\pm \sqrt{y-1}</mrow>
      </md>. 
      Since <m>\sqrt{y-1}</m> is always nonnegative, and since we seek <m>x</m> lying in <m>D=(-\infty,0]</m>, we see that we must have <m>x=-\sqrt{y-1}</m>, and thus  
      <me>
        f^{-1}(y)=-\sqrt{y-1}
      </me>.
    </p>
  </solution>
</example>

<theorem xml:id="th_inverse_function">
  <title>Inverse function compendium</title>
  <statement>
    <p>
      Let <m>f</m> be one-to-one on its domain <m>D</m>,
      let <m>R</m> be the range of <m>f</m>,
      and let <m>f^{-1}</m> be the inverse of <m>f</m>.
      <ol marker="itemsep0pt">
        <li>
          <p>
            <m>f^{-1}(b)=a \iff b=f(a)</m>
            for all <m>b\in R</m>. 
          </p>
        </li>
        <li>
          <p>
            The domain of <m>f^{-1}</m> is <m>R</m>, the range of <m>f</m>;
            the range of <m>f^{-1}</m> is <m>D</m>, the domain of <m>f</m>.
          </p>
        </li>
        <li>
          <p>
            We have
            <mdn>
              <mrow xml:id="eq_inverse_prop1">f^{-1}(f(a))\amp =a \text{ for all }  a\in X</mrow>
              <mrow xml:id="eq_inverse_prop2">f(f^{-1}(b))\amp =b \text{ for all }  b\in Y</mrow>
            </mdn>.
          </p>
        </li>
        <li>
          <p>
            The point <m>P=(x,y)</m> is on the graph of <m>f</m> if and only if the point <m>Q=(y,x)</m> is on the graph of <m>f^{-1}</m>.
          </p>
        </li>
        <li>
          <p>
            The graph of <m>f^{-1}</m> is the reflection of the graph of <m>f</m> through the line <m>y=x</m>.
          </p>
        </li>
      </ol>
    </p>
  </statement>
</theorem>
<theorem xml:id="th_IFT">
  <title>Derivative formula for inverses</title>
  <statement>
    <p>
      Assume <m>f</m> is one-to-one and differentiable on the interval <m>I</m>,
      and that <m>f'(x)\ne 0</m> for all <m>x\in I</m>.
      Let <m>J</m> be the range of <m>f</m>. 
      <ol>
        <li>
          <p>
            The inverse function <m>f^{-1}</m> is differentiable on <m>J</m>.
          </p>
        </li>
        <li>
          <p>
            We have
            <men xml:id="eq_IFT">
              (f^{-1})'(b)=\frac{1}{f'(f^{-1}(b))}
            </men>
            for all <m>b\in J</m>.
          </p>
        </li>
      </ol>
    </p>
  </statement>
  <proof>
    <p>
      We will not prove (1), which is the more difficult part of this theorem. Assuming <m>(1)</m> is true, we prove (2) using the chain rule as follows. By (2) of <xref ref="th_inverse_function"/>, we have <m>f^{-1}(f(x))=x</m> for all <m>x</m> in the domain of <m>f</m>. Taking derivatives of both sides of this equation, we see that
      <md>
        <mrow> \frac{d}{dx} (f^{-1}(f(x)))=\frac{d}{dx} x\amp \implies (f^{-1})'(f(x))f'(x)=1 \amp \text{(chain rule)}</mrow>
        <mrow> \amp \implies f^{-1}(f(x))=\frac{1}{f'(x)} \amp (f'(x)\ne 0)</mrow> 
      </md>. 
      Equivalently, since for any <m>b\in J</m> we have <m>f^{-1}(b)=a</m> for some unique <m>a\in I</m> satisfying <m>f(a)=b</m>, we see that 
      <md>
        <mrow>(f^{-1})'(b) \amp = (f^{-1})'(f(a)) </mrow>
        <mrow> \amp = \frac{1}{f'(a)} \amp \text{(by above)}</mrow>
        <mrow> \amp = \frac{1}{f'(f^{-1}(b))} \amp (a=f^{-1}(b))</mrow>
      </md>.
    </p>
  </proof>
</theorem>
<algorithm xml:id="proc_IFT">
  <title>Computing <m>(f^{-1})'(b)</m></title>
  <statement>
    <p>
      Let <m>f</m> be one-to-one on its domain <m>D</m>, let <m>R</m> be the range of <m>f</m>, and let <m>f^{-1}</m> be the inverse function of <m>f</m>. Given <m>b\in R</m>, to compute <m>(f^{-1})'(b)</m>, proceed as follows. 
      <ol>
        <li>
          <p>
            Compute <m>f^{-1}(b)=a</m>. This is often done by inspection: <ie/>,  by finding the unique <m>a</m> such that <m>f(a)=b</m>. 
          </p>
        </li>
        <li>
          <p>
            Compute <m>f'(x)</m>. 
          </p>
        </li>
        <li>
          <p>
            Use <xref ref="eq_IFT"/> to conclude <m>(f^{-1})'(b)=1/f'(f^{-1}(b))=1/f'(a)</m>. 
          </p>
        </li>
      </ol>
    </p>
  </statement>
</algorithm>
<example xml:id="eg_inverse_derivative">
  <title>Derivative of inverse</title>
  <statement>
    <p>
      Let <m>f</m> be defined as <m>f(x)=x^5+x^3+3x-5</m> on the domain <m>D=\R</m> of all real numbers.
      <ol>
        <li>
          <p>
            Show that <m>f</m> has an inverse function.
          </p>
        </li>
        <li>
          <p>
            Plot three points on the graph of <m>f^{-1}</m>.
          </p>
        </li>
        <li>
          <p>
            Compute <m>(f^{-1})'(-5)</m> and <m>(f^{-1})'(-10)</m>.
          </p>
        </li>
      </ol>
    </p>
  </statement>
  <solution>
    <p>
      <ol>
        <li>
          <p>
            Since <m>f'(x)=5x^4+3x^2+3</m> is clearly positive for all <m>x\in \R</m>, we see that <m>f</m> is increasing on its domain, and hence is one-to-one. Thus <m>f</m> has an inverse function. 
          </p>
        </li>
        <li>
          <p>
            Short of actually plotting points, we can at least produce a table of values for <m>f^{-1}</m> using a table of values of <m>f</m>, using (4) of <xref ref="th_inverse_function"/>.
            <md>
              <mrow>  
                \begin{array}{c|c}
                x\amp f(x) \\
                \hline 
                -1\amp -10\\
                0 \amp -5 \\
                1 \amp -2
                \end{array}
                
                \amp\implies  
              
                \begin{array}{c|c}
                x\amp f^{-1}(x) \\
                \hline 
                -10\amp -1\\
                -5 \amp 0 \\
                 -2\amp 1
                \end{array}
              </mrow>
            </md>
          </p>
        </li>
        <li>
          <p>
            For general <m>b</m> in the domain of <m>f^{-1}</m> (or equivalently, range of <m>f</m>), we have by <xref ref="th_IFT"/> 
            <md>
              <mrow>f^{-1}(b) \amp = \frac{1}{f'(f^{-1}(b))}</mrow>
              <mrow> \amp = \frac{1}{5(f^{-1}(b))^4+3(f^{-1}(b))^2+3} \amp (f'(x)=5x^4+3x^2+3)</mrow>
            </md>.
            Thus to compute <m>(f^{-1})'(-5)</m> and <m>(f^{-1})'(-10)</m>, it remains only to compute <m>f^{-1}(-5)</m> and <m>f^{-1}(-10)</m> and plug these into the last expression above. We see using our table of values in (b) that <m>f^{-1}(-5)=0</m> and <m>f^{-1}(-10)=-1</m>. Thus
            <md>
              <mrow>(f^{-1})'(-5) \amp = \frac{1}{(5\cdot 0+3\cdot 0+3)}=\frac{1}{3} </mrow>
              <mrow>(f^{-1})'(-10) \amp = \frac{1}{(5\cdot (-1)^4+3\cdot (-1)^2+3)}=\frac{1}{7} </mrow>
            </md>.
          </p>
        </li>
      </ol>
    </p>
  </solution>
</example>
</section>