<section>
    <title>Integration strategies</title>
    <introduction>
      <p>
        Having introduced a wealth of new derivative/integral formulas and rules,
        we now take a moment to give an overview of our integration techniques,
        and apply them in combination with some algebraic methods to solving integrals in the wild.
      </p>
    </introduction>
      <theorem xml:id="th_integral_formulas">
        <title>Idefinite integral compendium</title>
        <statement>
          <p>
            We collect here our various derivative/antiderivative formulas.
            <md>
              <mrow>\frac{d}{dx} x^r=rx^{r-1}\amp  \iff \int x^r \, dx=\frac{1}{r+1}x^{r+1}+C, r\ne -1</mrow>
              <mrow>\frac{d}{dx} \sin x=\cos x\amp  \iff \int\cos x \, dx=\sin x+C</mrow>
              <mrow>\frac{d}{dx}\cos x=-\sin x \amp  \iff \int \sin x \, dx=-\cos x+C</mrow>
              <mrow>\frac{d}{dx}\tan x=\sec^2x \amp  \iff \int \sec^2 x \, dx=\tan x+C</mrow>
              <mrow>\frac{d}{dx}\cot x=-\csc^2x \amp  \iff \int \csc ^2x\, dx=-\cot x+C</mrow>
              <mrow>\frac{d}{dx}\sec x=\sec x\tan x \amp  \iff \int \sec x\tan x \, dx=\sec x+C</mrow>
              <mrow>\frac{d}{dx}\csc x=-\csc x\cot x \amp  \iff \int\csc x\cot x \, dx=-\csc x+C</mrow>
              <mrow>\frac{d}{dx}\ln\vert x\vert=\frac{1}{x} \amp  \iff \int\frac{1}{x} \, dx=\ln\vert x\vert+C</mrow>
              <mrow>\frac{d}{dx}\ln\vert \cos x \vert=-\tan x \amp  \iff \int\tan x \, dx=-\ln\vert \cos x \vert+C=\ln\vert\sec x\vert+C</mrow>
              <mrow>\frac{d}{dx}\ln\vert \sin x\vert=\cot x \amp  \iff \int\cot x \, dx=\ln\vert \sin x\vert+C</mrow>
              <mrow>\frac{d}{dx}\ln\vert \sec x+\tan x\vert=\sec x \amp  \iff \int\sec x \, dx=\ln\vert \sec x+\tan x\vert+C</mrow>
              <mrow>\frac{d}{dx}\ln\vert \csc x+\cot x\vert=-\csc x \amp  \iff \int\csc x \, dx=-\ln\vert \csc x+\cot x\vert+C</mrow>
              <mrow>\frac{d}{dx}e^x=e^x \amp  \iff \int e^x \, dx=e^x+C</mrow>
              <mrow>\frac{d}{dx}a^x=(\ln a)a^x \amp  \iff \int a^x \, dx=\frac{1}{\ln a}a^x+C</mrow>
              <mrow>\frac{d}{dx}\log_a \vert x\vert =\frac{1}{(\ln a)\, x} \amp  \iff \int \frac{1}{(\ln a)\, x} \, dx=\log_a\vert x\vert+C</mrow>
              <mrow>\frac{d}{dx} \arcsin x=\frac{1}{\sqrt{1-x^2}}\amp \iff \int \frac{1}{\sqrt{1-x^2}}\, dx=\arcsin x+C</mrow>
              <mrow>\frac{d}{dx} \arccos x=-\frac{1}{\sqrt{1-x^2}}\amp \iff \int \frac{1}{\sqrt{1-x^2}}\, dx=-\arccos x+C</mrow>
              <mrow>\frac{d}{dx} \arctan x=\frac{1}{1+x^2}\amp \iff \int \frac{1}{1+x^2}\, dx=\arctan x+C </mrow>
            </md>.
          </p>
        </statement>
      </theorem>
      <p>
        Each of the integral computations below will combine various integral formulas,
        substitution, and an algebraic method.
      </p>
      <example xml:id="eg_int_vertex">
        <title>Vertex form</title>
        <statement>
            <p>
                Compute <m>\displaystyle \int \frac{1}{x^2-6x+18}\, dx</m>. 
            </p>
        </statement>
        <solution>
            <p>
               We have 
               <md>
                <mrow> \int \frac{1}{x^2-6x+18}\, dx \amp = \int \frac{1}{(x-3)^2+9}\, dx </mrow>
                <mrow> \amp = \frac{1}{9}\int\frac{1}{((x-3)/3)^2+1}</mrow>
                <mrow> \amp =\frac{1}{3}\int \frac{1}{u^2+1} \amp (u=(x-3)/3, du=\frac{1}{3}dx)</mrow>
                <mrow> \amp = \arctan((x-3)/3)+C</mrow>
               </md>.
            </p>
        </solution>
      </example>  
    
    <example xml:id="eg_poly_div">
        <title>Polynomial division</title>
        <statement>
            <p>
                Compute <m>\displaystyle \int \frac{4x^3+3x+1}{4x^2+1}\, dx</m>.
            </p>
        </statement>
        <hint>
            <p>
              Use polynomial division with remainder.
            </p>
        </hint>
        <solution>
            <p>
                Using polynomial division with remainder, we find that 
                <me>
                  \frac{4x^3+3x+1}{4x^2+1}=x+\frac{2x+1}{4x^2+1}
                </me>,
                 and thus 
                 <md>
                  <mrow>\int \frac{4x^3+3x+1}{4x^2+1}\, dx  \amp = \int x+\frac{2x+1}{4x^2+1}\, dx </mrow>
                  <mrow> \amp = \int x+\frac{2x}{4x^2+1}+\frac{1}{4x^2+1}\, dx</mrow>
                  <mrow> \amp = \frac{1}{2}x^2+\frac{1}{4}\ln\abs{4x^2+1}+\frac{1}{2}\arctan(2x)+C</mrow>
                 </md>.                
            </p>
        </solution>
    </example>
      
    <example xml:id="eg_exp_subst">
        <title>Exponential substitution</title>
        <statement>
            <p>
                Compute <m>\displaystyle\int \frac{1}{e^x+e^{-x}}\, dx</m>. 
            </p>
        </statement>
        <solution>
            <p>
                We have 
                <md>
                  <mrow> \int \frac{1}{e^x+e^{-x}}\, dx \amp = \int \frac{1}{u+1/u}\cdot \frac{1}{u}\, du \amp (u=e^x, du=e^x dx\implies dx=\frac{1}{u}du) </mrow>
                  <mrow> \amp = \int \frac{1}{u^2+1}\, du</mrow>
                  <mrow> \amp = \arctan(e^x)+C</mrow>
                </md>.
            </p>
        </solution>
    </example>
        
    <example xml:id="eg_exp_subst_2">
        <title>Exponential substitution (again)</title>
        
        
        <statement>
            <p>
                Compute <m>\displaystyle \int \frac{3}{\sqrt{e^{2x}-2}}\, dx</m>. 
            </p>
        </statement>
        <solution>
            <p>
                We have 
                <md>
                  <mrow> \int \frac{3}{\sqrt{e^{2x}-2}}\, dx \amp = \int \frac{3}{e^x\sqrt{1-2e^{-2x}}} \amp
                    (e^{2x}=(e^x)^2, 1/e^{2x}=e^{-2x})</mrow>
                    <mrow> \amp = -\frac{3}{\sqrt{2}}\int \frac{1}{\sqrt{1-u^2}}\, du \amp (u=\sqrt{2}e^{-x}, du=-\sqrt{2}e^{-x}dx\implies dx=-\frac{1}{\sqrt{2}u}du)</mrow>
                    <mrow> \amp  = -\frac{3}{\sqrt{2}}\arcsin(\sqrt{2}e^{-x})+C</mrow>
                </md>.
            </p>
        </solution>
    </example>
    
    <example xml:id="eg_trig_ident">
        <title>Trig identity</title>
        <statement>
            <p>
                Compute <m>\displaystyle \int_0^{\pi/3}\sin^2(2x)\cos(3x) \, dx</m>.
            </p>
        </statement>
        <hint>
            <p>
                Make use of some of the following product-to-sum identities.
                <md>
                  <mrow>\cos\theta\cos\phi\amp =\frac{\cos(\theta-\phi)+\cos(\theta+\phi)}{2}</mrow>
                  <mrow>\sin\theta\sin\phi\amp =\frac{\cos(\theta-\phi)-\cos(\theta+\phi)}{2}</mrow>
                  <mrow>\sin\theta\cos\phi\amp = \frac{\sin(\theta-\phi)+\sin(\theta+\phi)}{2}</mrow>
                  <mrow>\cos^2\theta\amp =\frac{1+\cos2\theta}{2}</mrow>
                  <mrow>\sin^2\theta\amp =\frac{1-\cos2\theta}{2}</mrow>
                </md>
            </p>
        </hint>
        <solution>
            <p>
                We have 
                <md>
                  <mrow> \int_0^{\pi/3}\sin^2(2x)\cos(3x) \, dx \amp = \int_0^{\pi/3}\frac{1}{2}(1-\cos(4x))\cos(3x) \, dx </mrow>
                  <mrow> \amp = \frac{1}{2}\int_0^{\pi/3}\cos(3x)-\cos(4x)\cos(3x)\, dx</mrow>
                  <mrow> \amp =\frac{1}{6}\sin(3x)\vert_0^{\pi/3}-\frac{1}{2}\int\frac{1}{2}(\cos x+\cos(7x))\, dx </mrow>
                  <mrow> \amp = 0-\left( \frac{1}{4}\sin x+\frac{1}{28}\sin 7x\right)\Bigr\vert_0^{\pi/3}</mrow>
                  <mrow> \amp = -\left( \frac{\sqrt{3}}{8}+\frac{\sqrt{3}}{56}\right)</mrow>
                  <mrow> \amp = -\frac{\sqrt{3}}{7}</mrow>
                </md>.
            </p>
        </solution>
    </example>
    

  </section>