<section>
    <title>Integration by parts</title>
    <introduction>
        <p>
            The integration by parts technique is yet another instance of our <xref ref="mantra_integration_differentiation"/>. In this case we take the familiar product rule of differentiation 
            <men xml:id="eq_prod_rule">
                (fg)' =f'g+fg'
            </men>,
        reexpress it algebraically as 
        <mdn>
            <mrow>f'g \amp = (fg)'-fg'</mrow>
        </mdn>,
        and then integrate both sides to conclude 
        <mdn>
            <mrow>\int f(x)g'(x)\, dx \amp = \int (f(x)g(x))'\, dx- \int f'(x)g(x)\, dx</mrow>
            <mrow> \amp = f(x)g(x)-\int f(x)g'(x)\, dx</mrow>
        </mdn>.
        We have just given a proof of what is called the <xref ref="th_int_by_parts" text="custom">integration by parts</xref> rule.  
        </p>
    </introduction>
      <theorem xml:id="th_int_by_parts">
        <title>Integration by parts</title>
        <statement>
          <p>
            Let <m>u</m> and <m>v</m> be continuously differentiable functions on an interval <m>I</m> containing the interval <m>[a,b]</m>.
            <ol>
              <li>
                <title>Indefinite integral form</title>
                <p>
                  We have
                  <men xml:id="eq_int_by_parts_ind">
                    \int u(x)v'(x)\, dx= u(x)v(x)-\int u'(x)v(x)\, dx
                  </men>.
                </p>
              </li>
              <li>
                <title>Definite integral form</title>
                <p>
                  We have
                  <men xml:id="eq_int_by_parts_def">
                    \int_a^b u(x)v'(x)\, dx= u(x)v(x)\Bigr\vert_a^b-\int_a^b u'(x)v(x)\, dx
                  </men>.
                </p>
              </li>
            </ol>
          </p>
        </statement>
      </theorem>
    
      <algorithm xml:id="proc_int_by_parts">
        <title>The art of by parts</title>
        <statement>
          <p>
            To use the integration by parts technique on an integral of the form <m>\displaystyle\int f(x)g(x)\, dx</m> proceed as follows:
            <ol>
              <li>
                <title>Who is <m>u</m>, and who <m>v'</m>?</title>
                <p>
                  Declare one of <m>f</m> and <m>g</m> to be <m>u</m> and the other to be <m>v'</m>.
                  The mnemonic device LIPET ((L)og, (I)nverse trig, (P)olynomial/radical, (E)xponent, (T)rig) often leads to a useful choice of <m>u</m>.
                </p>
              </li>
              <li>
                <title>Assemble ingredients</title>
                <p>
                  Suppose without loss of generality that we have chosen <m>u=f</m> and <m>v'=g</m>.
                  Then compute the derivative <m>f'</m> of <m>f</m> and compute an
                  <em>antiderivative</em> <m>G</m> of <m>g</m>:
                  <image xml:id="im_int_by_parts" width="100%">
                    <description>Integration by parts diagram</description>
                    <latex-image>
                        \begin{tikzcd}
                        u(x)=f(x) \ar[d,bend right=80,"\text{ compute derivative } "'] \amp  v'(x)=g(x) \ar[d,bend left=80,"\text{ compute antiderivative } "]\\ u'(x)=f'(x) \amp  v(x)=G(x)
                        \end{tikzcd}
                      </latex-image>
                  </image>
                </p>
              </li>
              <li>
                <title>Apply by parts rule</title>
                <p>
                Using the ingredients assembled in Step 2, we have 
                  <md>
                    <mrow>\int \underset{u}{f(x)}\underset{v'}{g(x)}\, dx\amp = \underset{u}{f(x)}\underset{v}{G(x)}-\int \underset{u'}{f'(x)}\underset{v}{G(x)}\, dx</mrow>
                  </md>.
                </p>
              </li>
            </ol>
          </p>
        </statement>
    </algorithm>
    <example xml:id="eg_by_parts_1">
        <title>Classic by parts</title>
        <statement>
            <p>
                Compute <m>\displaystyle\int_0^1 xe^{-x}\, dx</m> 
            </p>
        </statement>
        <solution>
            <p>
                <md>
                  <mrow> \int_0^1 xe^{-x}\, dx\amp = -xe^{-x}\Bigr\vert_0^1+\int_0^1 e^{-x}\, dx \amp (u=x, v'=e^{-x}) </mrow>
                  <mrow> \amp = -\frac{1}{e}-e^{-x}\Bigr\vert_0^1</mrow>
                  <mrow> \amp = 1-\frac{2}{e}</mrow>
                </md>. 
            </p>
        </solution>
    </example>
      <algorithm xml:id="proc_int_workflow">
        <title>Integration workflow</title>
        <statement>
          <p>
            For many integral computations it will be clear whether to use a formula,
            substitution, or integration by parts.
            When it is not clear how to proceed,
            the following  workflow might be helpful.
            <ol marker="0">
              <li>
                <title>Algebra and formulas</title>
                <p>
                  If possible, use an integration formula,
                  perhaps after some simple algebraic preparation.
                  Otherwise, move to (1).
                </p>
              </li>
              <li>
                <title>Substitution</title>
                <p>
                  Evaluate whether a substitution could transform the integral into one where (0) applies.
                  If not promising, move to (2).
                </p>
              </li>
              <li>
                <title>By parts</title>
                 <p>
                  Evaluate whether the integral is amenable to a by parts approach.
                  You may want to mentally run through a couple of choices of ``who is <m>u</m>,
                  and who <m>v'</m>". If not promising, move to (3).
                </p>
              </li>
              <li>
                <title>Creative algebra</title>
                <p>
                  Consider more creative algebraic techniques,
                  including trigonometric identities.
                  If applicable, return to (0).
                </p>
              </li>
            </ol>
          </p>
        </statement>
    </algorithm>
    <p>
        The following integrals can all be computed using by parts. However, for some of these byou might also explore whether substitution could serve as a useful technique. 
    </p>
     <example xml:id="eg_by_parts_2">
        <title>Iterated by parts</title>
        <statement>
            <p>
                <m>\displaystyle \int x^2 e^x\, dx</m>
            </p>
        </statement>
        <solution>
            <p>
                <md>
                  <mrow> \int x^2 e^x\, dx \amp = x^2e^{x}-2\int xe^{x}\, dx \amp (u=x^2, v'=e^x) </mrow>
                  <mrow> \amp = x^2e^x-2(xe^x-\int e^{x}) \amp (u=x, v'=e^x)</mrow>
                  <mrow> \amp = x^2e^x-2xe^x+2e^x+C</mrow>
                </md>. 
            </p>
        </solution>
     </example>
    
    <example xml:id="eg_by_parts_4">
        <title>Surprising by parts</title>
        <statement>
            <p>
                Compute <m>\displaystyle\int \ln \vert x\vert\, dx</m>
              </p>
        </statement>
        <solution>
            <p>
                We have <m>\ln x=\ln \abs{x}\cdot 1</m>. LIPET suggests trying <m>u=\ln \abs{x}</m>, <m>v'=1</m>: 
                <md>
                  <mrow>\int \ln \vert x\vert\, dx \amp = x\ln\abs{x}-\int \cancel{x}\cdot \frac{1}{\cancel{x}}\, dx 
                    \amp (u=\ln \abs{x}, v'=1)
                  </mrow>
                  <mrow> \amp = x\ln\abs{x}-\int 1\, dx</mrow>
                  <mrow> \amp = x\ln\abs{x}-x+C</mrow>
                </md>.
            </p>
        </solution>
    </example>  
    <example xml:id="eg_by_parts_5">
        <title>Rational function</title>
        <statement>
            <p>
                Compute <m>\displaystyle\int \frac{x^3}{x^2+1}\, dx</m>
              </p>
        </statement>
        <solution>
            <p>
             Using by parts with <m>u=x^2</m> and <m>v'=\frac{x}{x^2+1}</m>, we have 
             <md>
              <mrow> \int \frac{x^3}{x^2+1}\, dx\amp= \frac{1}{2}x^2\ln \abs{x^2+1}-\int x\ln\abs{x^2+1}\, dx </mrow>
              <mrow> \amp = \frac{1}{2}x^2\ln\abs{x^2+1}-\frac{1}{2}\int \ln \abs{u}\, du \amp (u=x^2+1, du=2xdx)</mrow>
              <mrow> \amp = \frac{1}{2}x^2\ln\abs{x^2+1}-\frac{1}{2}(u\ln\abs{u}-u)+C \amp (<xref ref="eg_by_parts_4"/>)</mrow>
              <mrow> \amp = \frac{1}{2}x^2\ln\abs{x^2+1}-\frac{1}{2}(x^2+1)\ln\abs{x^2+1}+\frac{1}{2}(x^2+1)+C </mrow>
              <mrow> \amp = \frac{1}{2}(x^2+1)-\ln\abs{x^2+1}+C</mrow>
             </md>. 
             Alternatively, using the substitution <m>u=x^2+1</m>, we have 
             <md>
              <mrow> \int \frac{1}{2}\frac{x^3}{x^2+1}\, dx \amp = \frac{1}{2}\int \frac{u-1}{u}\, du \amp (u=x^2+1, du=2xdx) </mrow>
              <mrow> \amp = \frac{1}{2}\int 1-\frac{1}{u}\, du </mrow>
              <mrow> \amp = \frac{1}{2}(x^2+1)-\ln\abs{x^2+1}+C</mrow>
             </md>.
             As a third alternative, we could use <em>polynomial division</em> to write <m>\frac{x^3}{x^2+1}=x-\frac{x}{x^2+1}</m>, and then conclude
             <me>
              \int \frac{x^3}{x^2+1}\, dx=\int x-\frac{x}{x^2+1}\, dx=\frac{1}{2}x^2-\ln\abs{x^2+1}+C
             </me>.
             Note that the answer here differs from the previous two by the constant <m>\frac{1}{2}</m>, which of course is not a problem. 

             
             
            </p>
        </solution>
    </example>  
    <example xml:id="eg_by_parts_6">
        <title>Inverse trig</title>
        <statement>
            <p>
                Compute <m>\displaystyle\int \arctan x\, dx</m>
            </p>
        </statement>
        <solution>
            <p>
               If using by parts, LIPET suggests the choice <m>u=\artcan x</m>, <m>v'=1</m>: 
               <md>
                <mrow> \int \arctan x\, dx \amp = x\arctan x-\int \frac{x}{x^2+1}\, dx </mrow>
                <mrow> \amp = x\arctan x-\frac{1}{2}\ln\abs{x^2+1}+C</mrow>
               </md>.
              </p>
        </solution>
    </example>
    <example xml:id="eg_by_parts_7">
        <title>By parts and algebra</title>
        <statement>
            <p>
                Compute <m>\int e^x\cos x\, dx</m>
              </p>
        </statement>
        <solution>
            <p>
                Here is an example where it looks like we are in danger of entering an infinite regress, but where a minus sign comes to our rescue. We have 
                <md>
                  <mrow> \int e^x\cos x\, dx\amp = e^x\sin x-\int e^x\sin x \amp (u=e^x, v'=\cos x) </mrow>
                  <mrow> \amp = e^x\sin x-(-e^x\cos x+\int e^x\cos x\, dx) \amp (u=e^x,v'=\sin x)</mrow>
                  <mrow> \amp = e^x\sin x+e^x\cos x-\int e^x\cos x\, dx</mrow>
                </md>.
                We've shown that 
                <me>
                  \int e^x\cos x\, dx=e^x\sin x+e^x\cos x-\int e^x\cos x\, dx
                </me>.
                Using algebra, it follows that 
                <me>
                  2\int e^x\cos x=e^x\sin x+e^x\cos x+C
                </me>,
                or
                <me>
                  \int e^x\cos x\, dx=\frac{1}{2}(e^x\sin x+e^x\cos x)+D
                </me>.
            </p>
        </solution>
    </example>
  </section>