<?xml version="1.0" encoding="UTF-8"?>

<section xml:id="s_inverse_trig" xmlns:xi="http://www.w3.org/2001/XInclude">
    <title>Inverse trigonometric functions</title>

    <definition xml:id="d_inverse_trig">
        <title>Inverse trigonometric functions</title>
      <statement>
        <p>
          The following are examples of what are called
          <em>inverse trigonometric functions</em>.
          <ul>
            <li>
              <p>
                On the restricted domain <m>[-\pi/2, \pi/2]</m> the function
                <m>f(x)=\sin x</m> is one-to-one, with range <m>[-1,1]</m>.
                The inverse function of <m>f</m> restricted to this domain is called the
                <em>arcsine function</em>,
                denoted <m>f^{-1}(x)=\arcsin x</m>.
              </p>
            </li>
            <li>
              <p>
                On the restricted domain <m>[0, \pi]</m> the function
                <m>g(x)=\cos x</m> is one-to-one, with range <m>[-1,1]</m>.
                The inverse function of <m>g</m> restricted to this domain is called the
                <em>arccosine function</em>,
                denoted <m>g^{-1}(x)=\arccos x</m>.
              </p>
            </li>
            <li>
              <p>
                On the restricted domain <m>(-\pi/2, \pi/2)</m> the function <m>h(x)=\tan x</m> is one-to-one,
                with range <m>(-\infty, \infty)</m>.
                The inverse function of <m>h</m> restricted to this domain is called the
                <em>arctangent function</em>,
                denoted <m>h^{-1}(x)=\arctan x</m>.
              </p>
            </li>
          </ul>
        </p>
      </statement>
    </definition>
    <remark>
      <p>
        Occasionally an alternative notation is used to denote inverse trigonometric functions: namely, 
        <md>
          <mrow>\arcsin x \amp = sin^{-1}x \amp \arccos x\amp =\cos^{-1} x \amp \arctan x\amp=\tan^{-1} x</mrow>    
        </md>.
        We will avoid this notation as it misleadingly suggests that the inverse trigonometric functions are <em>reciprocals</em> of the corresponding trigonometric functions. They are not! 
      </p>
    </remark>
    
    <theorem xml:id="th_inverse_trig_props">
        <title>Properties of inverse trigonometric functions</title>
        <statement>
          <ul>
            <li>
              <p>
                The function <m>\arcsin</m> is an increasing function with domain <m>[-1,1]</m> and range <m>[0,\pi]</m>.
                It satisfies the following properties:
                <mdn>
                  <mrow xml:id="eq_arcsin">\arcsin(x)=\theta \amp \iff \sin\theta=x \text{ and }  -\pi/2\leq \theta\leq \pi/2</mrow>
                  <mrow xml:id="eq_arcsin_sin">\arcsin(\sin \theta)\amp =\theta \text{ for all }  -\pi/2\leq \theta\leq \pi/2</mrow>
                  <mrow xml:id="eq_sin_arcsin">\sin(\arcsin x)\amp =x \text{ for all }  -1\leq x\leq 1</mrow>
                </mdn>.
              </p>
            </li>
            <li>
              <p>
                The function <m>\arccos</m> is a decreasing function with domain <m>[-1,1]</m> and range <m>[0,\pi]</m>.
                It satisfies the following properties:
                <mdn>
                  <mrow xml:id="eq_arccos">\arccos(x)=\theta \amp \iff \cos\theta=x \text{ and }  0\leq \theta\leq \pi</mrow>
                  <mrow>\arccos(\cos \theta)\amp =\theta \text{ for all }  0\leq \theta\leq \pi</mrow>
                  <mrow>\cos(\arccos x)\amp =x \text{ for all }  -1\leq x\leq 1</mrow>
                </mdn>.
              </p>
            </li>
            <li>
              <p>
                The function <m>\arctan</m> is an increasing function with domain
                <m>(-\infty, \infty)</m> and range <m>(-\pi/2, \pi/2)</m>.
                It satisfies the following properties:
                <mdn>
                  <mrow xml:id="eq_arctan">\arctan(x)=\theta \amp \iff \tan\theta=x \text{ and }  -\pi/2\lt  \theta\lt  \pi/2</mrow>
                  <mrow>\arctan(\tan \theta)\amp =\theta \text{ for all }  -\pi/2\lt  \theta\lt  \pi/2</mrow>
                  <mrow>\tan(\arctan x)\amp =x \text{ for all }  x</mrow>
                  <mrow>\lim_{x\to\infty}\arctan x\amp =\pi/2,\hspace{5pt} \lim_{x\to-\infty}\arctan x=-\pi/2</mrow>
                </mdn>
              </p>
            </li>
          </ul>
        </statement>
    </theorem>
    <example xml:id="eg_inverse_trig_compute">
      <title>Computing with inverse trig functions</title>
      <statement>
              <p>
                Compute the following values of trigonometric functions by hand.
                <ol>
                  <li>
                    <p>
                      <m>\displaystyle\arcsin(-1)</m>
                    </p>
                  </li>
                  <li>
                    <p>
                      <m>\displaystyle\arccos(-\sqrt{2}/2)</m>
                    </p>
                  </li>
                  <li>
                    <p>
                      <m>\displaystyle\arctan(-1/\sqrt{3})</m>
                    </p>
                  </li>
                  <li>
                    <p>
                      <m>\displaystyle\arcsin\left(\sin\left(\frac{10\pi}{11}\right)\right)</m> <em>Hint</em>.
                      The answer is not <m>10\pi/11</m>.
                    </p>
                  </li>
                </ol>
              </p>
      </statement>
      <solution>
          <p>
             <ol>
              <li>
                <p>
                  Common mistake: <m>\arcsin(-1)\ne 3\pi/2</m>. Why? By definition, the outputs of <m>\arcsin</m> lie in the interval <m>[-\pi/2, \pi/2]</m>. Instead, 
                  using <xref ref="eq_arcsin"/>, we have <m>\arcsin(-1)=\theta</m> if and only if <m>\sin \theta=-1</m> and <m>-\pi/2\leq \theta\leq \pi/2</m>. The unique <m>\theta</m> satisfying these two conditions is <m>\theta=-\pi/2</m>. We conclude that <m>\arcsin(-1)=-\pi/2</m>. 
                </p>
              </li>
              <li>
                <p>
                  Using <xref ref="eq_arcsin"/>, we have <m>\arccos(-\sqrt{2}/2)=\theta</m> if and only if <m>\cos \theta=-\sqrt{2}/2</m> and <m>0/\leq \theta\leq \pi</m>. The unique <m>\theta</m> satisfying these two conditions is <m>\theta=3\pi/4</m>. We conclude that <m>\arccos(-\sqrt{2}/2)=3\pi/4</m>. 
                </p>
              </li>
              <li>
                <p>
                  Using <xref ref="eq_arctan"/>, we have <m>\arctan(-1/\sqrt{3})=\theta</m> if and only if <m>\tan \theta=-1/\sqrt{3}</m> and <m>-\pi/2 &lt; \theta &lt; \pi/2</m>. Since <m>\theta=-\pi/6</m> is the unique angle satifying these two conditions, we conclude that that <m>\arctan(-1/\sqrt{3})=-\pi/6</m>. 
                </p>
              </li>
              <li>
                <p>
                  Recall that <m>\sin(\theta)=\sin (\pi-\theta)</m> for any <m>\theta\in \R</m>. (You can convince yourself of this either by drawing a unit circle picture, or by using the difference identity for <m>\sin</m>.) It follows that 
                  <md>
                    <mrow>\arcsin(\sin(10\pi/11)) \amp =\arcsin(\sin(\pi-10\pi/11))</mrow>
                    <mrow> \amp = \arcsin(\sin (\pi /11))</mrow>
                    <mrow> \amp = \frac{\pi}{11} \amp (<xref ref="eq_arcsin_sin"/>, -\frac{\pi}{2}\leq \frac{\pi}{11}\leq\frac{\pi}{2})</mrow>
                  </md>.
                </p>
              </li>
             </ol> 
          </p>
      </solution>
  </example>
    <example xml:id="eg_inverse_trig_solve">
        <title>Solving trig equations</title>
        <statement>
            <p>
                Find all solutions to the following trigonometric equations lying within the interval <m>[0,2\pi]</m>.
                You may express your answer in terms of values of inverse trigonometric functions.
                <ol>
                  <li>
                    <p>
                      <m>\displaystyle 3\sin 2\theta +4=6</m>
                    </p>
                  </li>
                  <li>
                    <p>
                      <m>\displaystyle \tan (\theta+\pi)=-10</m>
                    </p>
                  </li>
                </ol>
              </p>
        </statement>
        <solution>
            <p>
                
            </p>
        </solution>
    </example>
    <theorem xml:id="th_inverse_trig_derivative">
        <title>Derivatives of inverse trig functions</title>
      <statement>
        <p>
          The following derivative/antiderivative formulas hold:
          <mdn>
            <mrow xml:id="eq_arcsin_der">\frac{d}{dx} \arcsin x=\frac{1}{\sqrt{1-x^2}}\amp \iff \int \frac{1}{\sqrt{1-x^2}}\, dx=\arcsin x+C \amp \text{ (for all \(x\) in \((-1,1)\)) }</mrow>
            <mrow xml:id="eq_arccos_der">\frac{d}{dx} \arccos x=-\frac{1}{\sqrt{1-x^2}}\amp \iff \int \frac{1}{\sqrt{1-x^2}}\, dx=-\arccos x+C \amp \text{ (for all \(x\) in \((-1,1)\)) }</mrow>
            <mrow xml:id="eq_arctan_der">\frac{d}{dx} \arctan x=\frac{1}{1+x^2}\amp \iff \int \frac{1}{1+x^2}\, dx=\arctan x+C \amp \text{ (for all \(x\)) } </mrow>
          </mdn>.
        </p>
      </statement>
      <proof>
        <p>
          We prove <xref ref="eq_arcsin_der"/> and <xref ref="eq_arctan"/>; the proof of <xref ref="eq_arccos_der"/> proceeds along similar lines. 
        </p>
        <proof>
          <title>Proof of <xref ref="eq_arcsin_der"/>  </title>
          <p>
            Let <m>f(x)=\sin x</m> restricted to the domain <m>D=[-\pi/2, \pi/2]</m>, and let <m>f^{-1}(x)=\arcsin x</m>. Using <xref ref="th_IFT"/>, we have 
            <md>
              <mrow>\frac{d}{dx} \arcsin x \amp = \frac{1}{f'(\arcsin x)}</mrow>
              <mrow> \amp = \frac{1}{\cos(\arcsin x)}</mrow>
              <mrow> \amp = \frac{1}{\sqrt{1-x^2}</mrow>
            </md>.
            The last step here is perhaps the most interesting, and follows from the fact that <m>\cos(\arcsin x)=\sqrt{1-x^2}</m> for any <m>x\in [-1,1]</m>. Why is this true? Set <m>\arcsin x=\theta</m>, an angle lying in <m>[-\pi/2,\pi/2]</m>. Using the fact that <m>\sin \theta=x</m>, we can draw a unit circle picture like the one below. Since the vertical leg of the right triangle there has length <m>\abs{x}</m>, the horizontal leg has length <m>\sqrt{1-\abs{x}^2}=\sqrt{1-x^2}</m>. Since this length is equal to the <m>x</m>-coordinate of the point <m>P</m> below, we have <m>\cos \theta=\sqrt{1-x^2}</m> and thus <m>\cos(\arcsin x)=\sqrt{1-x^2}</m>, as claimed.   
            <image source="images/arcsin_der.png" width="75%">
              <description>Unit circle picture for arcsin derivative proof</description>
            </image>
          </p>
        </proof>
        <proof>
          <title>Proof of <xref ref="eq_arctan_der"/>  </title>
          <p>
            Let <m>f(x)=\tan x</m> restricted to the domain <m>D=(-\pi/2, \pi/2)</m>, and let <m>f^{-1}(x)=\arctan x</m>. Using <xref ref="th_IFT"/>, we have 
            <md>
              <mrow>\frac{d}{dx}\arctan x \amp = \frac{1}{f'(\arctan x)}</mrow>
              <mrow> \amp = \frac{1}{\sec^2 (\arctan x)}</mrow>
              <mrow> \amp = \frac{1}{(\tan(\arctan x))^2+1} \amp (\tan^2 x+1=\sec^2x)</mrow>
              <mrow> \amp = \frac{1}{x^2+1} \amp (\tan(\arctan x)=x)</mrow>
            </md>.
          </p>
        </proof>
      </proof>
    </theorem>
    <example xml:id="eg_inverse_trig_derivative">
        <title>Derivatives of inverse trig functions</title>
        
        <statement>
            <p>
                Find the equation of the tangent line to <m>f(x)=\arccos x</m> at <m>x=1/2</m>.
              </p>
        </statement>
        <solution>
            <p>
                
            </p>
        </solution>
    </example>

    <example xml:id="eg_inverse_trig_integral">
        <title>Integrating with inverse trig functions</title>
        <statement>
            <p>
                Compute the following integrals. 
                <ol>
                    <li>
                        <p>
                            <m>\displaystyle\lim_{x\rightarrow 1^{-}}\frac{\arccos(x^2)}{\sqrt{1-x}}</m>
                        </p>
                    </li>
                    <li>
                        <p>
                            <m>\displaystyle\int \frac{x+1}{\sqrt{1-(x+2)^2}}\, dx</m>
                        </p>
                    </li>
                </ol>
            </p>
        </statement>
        <solution>
            <p>
                
            </p>
        </solution>
    </example>
</section>