<?xml version="1.0" encoding="UTF-8"?>

<section xml:id="s_linear_diff_eq" xmlns:xi="http://www.w3.org/2001/XInclude">
    <title>First-order linear differential equations</title>
    <definition xml:id="d_lin_diff_eq">
        
        <title>First-order linear equation</title>
      <statement>
        <p>
          A <term>first-order linear differential equation</term>
          for the function <m>f</m> is a differential equation that can be written in the form
          <men xml:id="eq_lin_diff_eq">
            f'(x)+p(x)f(x)=q(x)
          </men>
          for some functions <m>p</m> and <m>q</m>. 
          Equation <xref ref="eq_lin_diff_eq"/> is called the
          <term>standard form</term> of the equation.
        </p>
      </statement>
    </definition>
    
    <definition xml:id="d_int_factor">
        <title>Integrating factor</title>
      <statement>
        <p>
          Consider a first-order linear equation with standard form
          <me>
            f'(x)+p(x)f(x)=q(x)
          </me>.
        </p>
        <p>
          An <term>integrating factor</term> for this equation is any function of the form
          <me>
            v(x)=e^{P(x)}
          </me>,
          where <m>P(x)</m> is an antiderivative of <m>p(x)</m>.
        </p>
        <p>
            As a somewhat liberal usage of indefinite integral notation, we sometimes write 
          <m>
            v(x)=e^{\int p(x)\, dx}
          </m>.
        </p>
      </statement>
    </definition>

    <algorithm xml:id="proc_lin_diff_eq">
        <title>Solving first-order linear equations</title>
      <statement>
        <p>
          Suppose <m>p, q</m> are continuous on the interval <m>I</m>.
          To solve the differential equation with standard form
          <men xml:id="eq_solve_diff_eq">
            f'(x)+p(x)f(x)=q(x), \ x\in I
          </men>,
          proceed as follows.
          <ol>
            <li>
              <p>
                Compute <m>\int p(x)\, dx=P(x)+C</m>.
              </p>
            </li>
            <li>
              <p>
                Set <m>v(x)=e^{P(x)}</m>.
              </p>
            </li>
            <li>
              <p>
                The function <m>f</m> is a solution of <xref ref="eq_solve_diff_eq"/> if and only if it is a solution of
                <men xml:id="eq_solve_aux_eq">
                  (v(x)f(x))'=v(x)q(x)
                </men>.
              </p>
            </li>
            <li>
              <p>
                Compute <m>\int v(x)q(x)\, dx=G(x)+C</m>.
                Since <m>G(x)+C</m> is the general solution of <xref ref="eq_solve_aux_eq"/>, the general solution of <xref ref="eq_solve_diff_eq"/> is
                <me>
                  f(x)=\frac{1}{v(x)}(G(x)+C)=\frac{G(x)}{v(x)}+\frac{C}{v(x)}
                </me>,
                where <m>C</m> is any constant.
              </p>
              <p>
                As a somewhat liberal usage of indefinite integral notation, we sometimes write 
                <m>
                  f(x)=\frac{1}{v(x)}\int v(x)q(x)\, dx
                </m>.
              </p>
            </li>
          </ol>
        </p>
      </statement>
    </algorithm>
<example xml:id="eg_exp_growth_revisited">
    <title>Exponential change revisited</title>

    <statement>
        <p>
            Use the integrating factor method to find the general solution to <m>y'=k y</m>,
            where <m>k</m> is any fixed nonzero constant.
          </p>
    </statement>
    <solution>
        <p>
            Observe that this differential equation is both linear and separable, but we are asked here to use the linear differential equation technique for solving The standard form of the differential equation is 
            <me>
              y'\underset{p(x)}{\underbrace{-k}}y=\underset{q(x)}{\underbrace{0}}
            </me>.
            Clearly, <m>P(x)=-kt</m> is an antiderivative of <m>p(x)=-k</m>, so we set 
            <me>v(x)=e^{-kt}</me>.
            Next we compute 
            <me>
              \int v(x)q(x)\, dx=\int 0\, dx= C
            </me>.
            Finally, we conclude that the general solution is 
            <me>
              f(x)=\frac{C}{v(x)}=\frac{C}{e^{-kx}}=Ce^{kx}
            </me>.
            This should come as no surprise: we have re-derived the general solution to the exponential change differential equation <m>y'=ky</m>.
        </p>
    </solution>
</example>
<example xml:id="eg_lin_diff_eq">
    <title>Non-separable example</title>
    <statement>
        <p>
            Find the general solution to the differential equation
            <me>
              (x^2+1)f'(x)-x=x^3-xf(x), \  x\in (-\infty, \infty)
            </me>.
          </p>
    </statement>
    <solution>
        <p>
            Following <xref ref="proc_lin_diff_eq"/> we first bring the differential equation into standard form: 
            <me>
              f'(x)+\underset{p(x)}{\underbrace{\frac{x}{x^2+1}}}f(x)=\frac{x^3+x}{x^2+1}=\underset{q(x)}{\underbrace{x}}
            </me>.
            We then compute 
            <me>
              \int p(x)\, dx=\int \frac{x}{x^2+1}\, dx=\frac{1}{2}\ln\vert x^2+1\vert+C=\frac{1}{2}\ln (x^2+1)+C
            </me>, 
            and thus set 
            <me>
              v(x)=e^{\frac{1}{2}\ln(x^2+1)}=\sqrt{x^2+1}
            </me>.
            Next, we compute 
           <me>
              \int v(x)q(x)\, dx=\int x\sqrt{x^2+1}, dx=\underset{G(x)}{\underbrace{\frac{1}{3}(x^2+1)}}+C
            </me>.
          Finally, we conclude that the general solution is given by 
          <me>
            f(x)=\frac{G(x)}{v(x)}+\frac{C}{v(x)}=\frac{1}{3}(x^2+1)+\frac{C}{\sqrt{x^2+1}}
          </me>.   
          Note in particular that setting <m>C=0</m>, we see that the polynomial <m>f(x)=\frac{1}{3}(x^2+1)</m> is a solution to the differential equation.                
        </p>
    </solution>
</example>
<example xml:id="eg_non_separable">
    <title>Initial value</title>
    <statement>
        <p>
            Consider the differential equation
            <me>
              (x-2)f'=e^{-x}-3f, \ x\in (-\infty, 2)
            </me>.
            <ol>
              <li>
                <p>
                  Find the general solution to the differential equation.
                </p>
              </li>
              <li>
                <p>
                  Find the solution satisfying <m>f(1)=-1</m>.
                </p>
              </li>
            </ol>
          </p>
    </statement>
    <solution>
        <p>
            First we bring the differential equation into standard form: 
            <me>
              f'+\underset{p(x)}{\underbrace{\frac{3}{x-2}}}f=\underset{q(x)}{\underbrace{\frac{e^{-x}}{x-2}}}
            </me>.
            Since <m>3\ln\abs{x-2}</m> is an antiderivative of <m>p(x)=3/(x-2)</m>, we set the integrating factor to be 
            <me>
              v(x)=e^{3\ln\abs{x-2}}=\abs{x-2}^3=-(x-2)^3
            </me>,
            where the minus sign arises due to the fact that we assume <m>x\leq 2</m>, and hence <m>x-2\leq 0</m>. Next we compute (using integration by parts twice)
            <me>
              \int v(x)q(x)\, dx=\int -(x-2)^2e^{-x}\, dx=(x-2)^2e^{-x}+2(x-2)e^{-x}+2e^{-x}+C=\underset{G(x)}{\underbrace{(x^2-2x+2)e^{-x}}}+C
            </me>.
            We conclude that the general solution is given by 
            <me>
              f(x)=\frac{G(x)}{v(x)}+\frac{C}{v(x)}=-\frac{x^2-2x+2}{(x-2)^3}e^{-x}-\frac{C}{(x-2)^3}
            </me>. 
            Finally, the condition <m>f(1)=-1</m> implies that 
            <me>
              -\frac{1}{(-1)}e^{-1}-\frac{C}{(-1)}=-1
            </me>,
            and thus 
            <me>
              C=-(e^{-1}+1)
            </me>.
            
        </p>
    </solution>
</example>


</section>