<?xml version="1.0" encoding="UTF-8"?>

<section xml:id="s_rational_functions" xmlns:xi="http://www.w3.org/2001/XInclude">
    <title>Rational functions</title>
<definition xml:id="d_rational_function">
    <title>Rational function</title>
    <statement>
        <p>
            A <term>rational function</term> is a function that can be expressed as a quotient of two polynomials. 
        </p>
    </statement>
</definition>

<theorem xml:id="th_poly_facts">
    <title>Polynomial facts</title>
    <statement>
      <p>
        <ol>
          <li>
            <title>Degree</title>
            <p>
              Suppose <m>f(x)=\anpoly</m> with <m>a_n\ne 0</m>.
              We call <m>n</m> the <term>degree</term>
              of <m>f</m>, denoted <m>\deg f</m>.
            </p>
          </li>
          <li>
            <title>Roots of polynomials</title>
            <p>
              A polynomial of degree <m>n</m> has at most <m>n</m> distinct roots.
            </p>
          </li>
          <li>
            <title>Equating coefficients</title>
            <p>
              Given polynomials <m>f(x)=\anpoly</m> and <m>g(x)=\bmpoly</m> where <m>a_n\ne 0</m> and <m>b_m\ne 0</m>, we have
              <me>
                f(x)=g(x) \iff n=m \text{ and }  a_i=b_i \text{ for all \(i\). }
              </me>
            </p>
          </li>
          <li>
            <title>Irreducible</title>
            <p>
              A nonzero polynomial is <term>irreducible</term>
              if it cannot be factored into two polynomials of smaller degree.
              If <m>f(x)</m> is an irreducible polynomial with real coefficients,
              then <m>\deg f=1</m> or <m>\deg f=2</m>.
            </p>
          </li>
        </ol>
      </p>
      </statement>
</theorem>

<theorem xml:id="th_partial_frac">
    <title>Partial fraction decomposition</title>
    <statement>
        <p>
          Let <m>p(x)/q(x)</m> be a rational function
          where <m>\deg p &lt;  \deg q</m>.
          <ul>
            <li>
              <p>
                If <m>q</m> factors into non-repeated linear factors as
                <me>
                  q(x)=D(x-a_1)(x-a_2)\cdots (x-a_r)
                </me>,
                then there is a unique choice of constants <m>A_1, A_2,\dots, A_r</m> such that
                <men xml:id="eq_part_decomp_1">
                  \frac{p(x)}{q(x)}=\frac{A_1}{x-a_1}+\frac{A_2}{x-a_2}+\cdots +\frac{A_r}{x-a_r}
                </men>.
              </p>
            </li>
            <li>
              <p>
                If <m>q(x)</m> factors into non-repeated irreducible linear and quadratic factors as
                <me>
                  q(x)=D(x-a_1)(x-a_2)\cdots (x-a_r)(x^2+b_1x+c_1)(x^2+b_2x+c_2)\cdots (x^2+b_sx+c_s)
                </me>,
                there there is a unique choice of constants <m>A_1,A_2,\dots, A_r, B_1,B_2,\dots, B_s, C_1, C_2,\dots, C_s</m> such that
                <men xml:id="eq_part_decomp_2">
                  \frac{p(x)}{q(x)}=\frac{A_1}{x-a_1}+\frac{A_2}{x-a_2}+\cdots +\frac{A_r}{x-a_r}+\frac{B_1x+C_1}{x^2+b_1x+c_1}+\frac{B_2x+C_2}{x^2+b_2x+c_2}+\cdots +\frac{B_sx+C_s}{x^2+b_sx+c_s}
                </men>.
              </p>
            </li>
          </ul>
        </p>
      </statement>
</theorem>

<algorithm xml:id="proc_partial_frac">
    <title>Partial fraction decomposition</title>
      <statement>
        <p>
          Let <m>f(x)</m> be a rational function. To compute the partial fraction decomposition of <m>f</m>, proceed as follows. 
        </p>
        <p>
          <ol>
            <li>
                <title>Polynomial division</title>
                <p>
                    Using polynomial division if necessary, write <m>f(x)=g(x)+p(x)/q(x)</m>, where <m>g</m>, <m>p</m> and <m>q</m> are polynomials, and <m>\deg p &lt;  \deg q</m>. 
                </p>
            </li>
                
              <li>
                <title>Factor</title>
                <p>
                  Factor <m>q(x)</m> into powers of distinct irreducible polynomials.</p>
                  <p>
                  <em>Factoring trick</em>.
                  If <m>q(x)</m> has integer coefficients and a leading coefficient equal to 1, then any integer roots of <m>q(x)</m> will be factors of the constant term.
                </p>
              </li>
              <li>
                <title>Polynomial equation with undetermined constants</title>
                <p>
                  Set up a partial fraction decomposition equation for <m>p(x)/q(x)</m> of form <xref ref="eq_part_decomp_1"/> or <xref ref="eq_part_decomp_2"/>.
                  Clear the denominators of both sides of the equation,
                  resulting in an identity between two polynomials.
                  The polynomial on the right will be expressed in terms of the unknowns
                  (<m>A_i</m>, <m>B_i</m>, etc.).
                </p>
            </li>
                <li>
                    <title>Solve for undetermined constants</title>
                    <p>
                        To solve for the undetermined constants (<m>A_i</m>, <m>B_i</m>,
                        etc.) set up and solve a linear system of equations using one of the following techniques.
                        <ol>
                          <li>
                              <p>
                                <em>Evaluate equality at choices of <m>x</m></em>.
                                Evaluate the polynomial equation at various explicit choices of <m>x</m>. 
                                When <m>q</m> factors as <m>q(x)=D(x-a_1)(x-a_2)\cdots (x-a_m)</m> where the roots <m>a_k</m> are distinct, then evaluating the polynomial equality at each of the choices <m>x=a_k</m> will allow you to solve directly for each undetermined constant in turn. 
                              </p>
                            </li>
                        <li>
                          <p>
                            <em>Equate coefficients</em>.
                            Express the polynomial on right in
                            <q>standard form</q>
                            by collecting like terms.
                            For the left and right polynomials to be equal,
                            their corresponding coefficients must all be equal.
                            This yields a system of equations in the unknowns (<m>A_i</m>,
                            <m>B_i</m>, etc.) that you must now solve.
                          </p>
                        </li>
                  
                </ol>
              </p>
              </li>
            </ol>
                      </p>
        
      </statement>
</algorithm>
<remark>
    <p>
        There is a more general statement of partial fraction decomposition for the case where the irreducible factors of <m>q</m> include repeated linear and/or quadratic terms, but we will not cover it. Consult the textbook if you are curious.
    </p> 
</remark>
<example xml:id="eg_rat_func_1">
    <title>Rational function</title>
    <statement>
        <p>
            Compute <m>\displaystyle\int \frac{x+2}{x^2-1}\, dx</m>
          </p>
    </statement>
    <solution>
        <p>
            We have 
            <md>
              <mrow> \frac{x+2}{x^2-1}=\frac{A}{x-1}+\frac{B}{x+1}\amp \implies x+2=A(x+1)+B(x-1) </mrow>
            </md>.
            Evaluating the right-hand side at <m>x=1</m> and <m>x=-1</m> yields 
            <md>
              <mrow>3 \amp = 2A</mrow>
              <mrow>1 \amp = -2B</mrow>
            </md>, 
            and thus <m>A=3/2</m>, <m>B=-1/2</m>. We conclude 
            <md>
              <mrow> \int \frac{x+2}{x^2-1}\, dx \amp= \int \frac{3}{2}\frac{1}{x+1}-\frac{1}{2}\frac{1}{x-1}\, dx </mrow>
              <mrow> \amp = \frac{3}{2}\ln\abs{x+1}-\frac{1}{2}\ln\abs{x-1}+C</mrow>
            </md>.
        </p>
    </solution>
</example>

<example xml:id="eg_rat_func_4">
    <title>Long division first</title>
    <statement>
        <p>
            Compute <m>\displaystyle\int \frac{x^2}{x^2+2x-1}\, dx</m>
          </p>
    </statement>
    <solution>
        <p>
            First perform polynomial division with remainder to write 
            <me>
              \frac{x^2}{x^2+2x-1}=1-\frac{2x-1}{x^2+2x-1}
            </me>.
            Next, we factor <m>x^2+2x-1=(x-\alpha)(x-\beta)</m>, where 
            <md>
              <mrow>\alpha \amp = -1+\sqrt{2} \amp \beta\amp =-1-\sqrt{2}</mrow>
            </md>.
            Now perform partial fraction decomposition
            <md>
              <mrow>\frac{2x-1}{(x-\alpha)(x-\beta)} \amp = \frac{A}{x-\alpha}+\frac{B}{x-\beta}</mrow>
              <mrow>2x-1 \amp = A(x-\beta)+B(x-\alpha)</mrow>
            </md>.
            Evaluating the last identity at <m>x=\alpha</m> and <m>x=\beta</m>, we conclude 
            <md>
              <mrow>2\alpha-1 \amp = A(\alpha-\beta)</mrow>
              <mrow>2\beta-1 \amp = B(\beta-\alpha)</mrow>
            </md>,
            or equivalently, 
            <md>
              <mrow>-3+2\sqrt{2} \amp = 2\sqrt{2}A</mrow>
              <mrow>-3-2\sqrt{2} \amp= -2\sqrt{2}B</mrow>
            </md>. 
            We conclude that <m>A=\frac{1}{2\sqrt{2}}(-3+2\sqrt{2})=\frac{4-3\sqrt{2}}{4}</m> and <m>B=\frac{1}{2\sqrt{2}}(-3-2\sqrt{2})=\frac{4+3\sqrt{2}}{4}</m>, and thus 
            <md>
              <mrow> \int \frac{x^2}{x^2+2x-1}\, dx \amp  = \int 1-\frac{4-3\sqrt{2}}{4}\frac{1}{x-\alpha}-\frac{4+3\sqrt{2}}{4}\frac{1}{x-\beta}\, dx</mrow>
              <mrow> \amp = x-\frac{4-3\sqrt{2}}{4}\ln\abs{x-(-1+\sqrt{2})}-\frac{4+3\sqrt{2}}{4}\ln\abs{x-(-1-\sqrt{2})}+C</mrow>
            </md>
            
        </p>
    </solution>
</example>




<example xml:id="eg_rat_func_3">
    <title>Three distinct roots</title>
    <statement>
        <p>
            Compute <m>\displaystyle\int\frac{x^2+1}{x^3+2x^2-x-2}\, dx</m>
          </p>
    </statement>
    <solution>
        <p>
           First we factor <m>q(x)=x^3+2x^2-x-2</m>. An integer root of <m>q(x)</m> must divide <m>2</m>, thus we investigate <m>\pm 1, \pm 2</m> as potential roots. Since <m>q(1)=1+1-1-2=0</m>, we see that <m>x=1</m> is a root of <m>q(x)</m> and thus <m>(x-1)</m> is a factor of <m>q(x)</m>. Performing polynomial division with remainder, we see that <m>q(x)=(x-1)(x^2+3x+2)</m>. Factoring the quadratic term further, we see that 
           <me>
            q(x)=(x-1)(x+1)(x+2)
           </me>.
           Now perform partial fractions: 
           <md>
            <mrow> \frac{x^2+1}{x^3+2x^2-x-2} \amp =\frac{A}{x-1}+\frac{B}{x+1}+\frac{C}{x+2}</mrow>
            <mrow>x^2+1 \amp = A(x+1)(x+2)+B(x-1)(x+2)+C(x-1)(x+1)</mrow>
           </md>.
           Evaluating this identity at <m>x=1, -1,-2</m>, we see that 
           <md>
            <mrow>2 \amp = 6A </mrow>
            <mrow>2 \amp = -2B</mrow>
            <mrow>5 \amp = 3C</mrow>
           </md>
           and thus <m>A=\frac{1}{3}, B=-1, C=\frac{5}{3}</m>. Thus 
           <md>
            <mrow>\int\frac{x^2+1}{x^3+2x^2-x-2}\, dx \amp = \frac{1}{3}\frac{1}{x-1}-\frac{1}{x+1}+\frac{5}{3}\frac{1}{x+2}\, dx </mrow>
            <mrow> \amp = \frac{1}{3}\ln\abs{x-1}-\ln\abs{x+1}+\frac{5}{3}\ln\abs{x+2}+C</mrow>
           </md>. 
        </p>
    </solution>
</example>

<example xml:id="eg_rat_func_2">
    <title>Two irreducible quadratics</title>
    <statement>
        <p>
            Compute <m>\displaystyle\int\frac{1}{x^4+3x^2+2}</m>
          </p>
    </statement>
    <solution>
        <p>
          First note that the denominator <m>q(x)=x^4+3x^2+2=(x^2)^2+3x^2+2=(x^2+1)(x^2+2)</m>, where <m>x^2+1</m> and <m>x^2+2</m> are both irreducible. Now perform partial fractions: 
          <md>
            <mrow>\frac{1}{x^4+3x^2+2} \amp = \frac{Ax+B}{x^2+1}+\frac{Cx+D}{x^2+2}</mrow>
            <mrow>1 \amp = (Ax+B)(x^2+2)+(Cx+D)(x^2+1)=(A+C)x^3+(B+D)x^2+(A+2C)x+B+2D</mrow>
          </md>. 
          Note that in this case we cannot evaluate the identity above at the roots of <m>x^2+1</m> and <m>x^2+2</m> since they have none (in the reals)! Instead we use (3) from <xref ref="th_poly_facts"/> and produce a linear system by equating the coefficients of two polynomials <m>(A+B)x^3+(B+D)x^2+(A+2C)x+(B+2D)</m> and <m>0x^3+0x^2+0x+1</m>:
          <mdn>
            <mrow xml:id="eq_1">A+C \amp = 0</mrow>
            <mrow xml:id="eq_2">B+D \amp = 0</mrow>
            <mrow xml:id="eq_3">2A+C \amp = 0</mrow>
            <mrow xml:id="eq_4">2B+D \amp = 1</mrow>
          </mdn>.
          Equations <xref ref="eq_1"/> and <xref ref="eq_3"/> together imply <m>A=C=0</m>. Equation <xref ref="eq_2"/> implies <m>B=-D</m>; equation <xref ref="eq_4"/> then implies <m>D=-1</m> and <m>B=1</m>. We conclude that 
          <me>
            \frac{1}{x^4+3x^2+2}=\frac{1}{x^2+1}-\frac{1}{x^2+2}
          </me>
          and thus 
          <md>
            <mrow>\int \frac{1}{x^4+3x^2+2}\, dx \amp = \int \frac{1}{x^2+1}-\frac{1}{x^2+2}\, dx </mrow>
            <mrow> = \int \frac{1}{x^2+1}-\frac{1}{2(x/\sqrt{2})^2+1)}\, dx </mrow>
            <mrow> \amp = \arctan(x)-\frac{\sqrt{2}}{2}\arctan(x/\sqrt{2})+C</mrow>
          </md>
        </p>
    </solution>
</example>

<example xml:id="eg_rat_func_5">
    <title>With substitution</title>
    <statement>
        <p>
            Compute <m>\displaystyle \frac{\sin \theta}{\cos^2\theta +\cos \theta-2}\, d\theta</m>
        </p>
    </statement>
    <solution>
        <p>
            Resist the temptation to apply partial fraction decomposition directly to the integrand! Since the integrand is <em>not</em> a rational function, <xref ref="th_partial_frac"/> does not apply. Instead we first do an obvious substitution:
            <md>
              <mrow> \int \frac{\sin \theta}{\cos^2\theta +\cos \theta-2}\, d\theta \amp 
                = -\int \frac{1}{u^2 +u-2}\, du  \amp (u=\cos\theta, du=-\sin\theta d\theta) </mrow>
                <mrow> \amp = -\int \frac{1}{3}\frac{1}{u-1}-\frac{1}{3}\frac{1}{u+2}\, du \amp (\text{part. frac. decomp.})</mrow>
                <mrow> \amp =\frac{1}{3}(\ln\abs{\cos\theta+2}-\ln\abs{\cos\theta-1})+C</mrow>
                <mrow> \amp = \ln\sqrt[3]{\abs{\frac{\cos\theta+2}{\cos\theta-1}}}+C \amp (\text{log. props.})</mrow>
            </md> .
        </p>
    </solution>
</example>


</section>