<?xml version="1.0" encoding="UTF-8"?>



<section xml:id="separable_diffeq" xmlns:xi="http://www.w3.org/2001/XInclude">
    <title>Separable differential equations</title>
    
    <definition xml:id="d_exp_grow_decay">
      <title>Exponential growth and decay</title>
      <statement>
        <p>
          Suppose the function <m>f(x)</m> satisfies the differential equation
          <men xml:id="eq_exp_change">
            f'(x)=k\, f(x)
          </men>,
          where <m>k</m> is a fixed constant.
        </p>
        <p>
          If <m>k&gt; 0</m> then <m>f(x)</m> is said to undergo
          <term>exponential growth</term>.
        </p>
        <p>
          If <m>k&lt; 0</m> then <m>f(x)</m> is said to undergo
          <term>exponential decay</term>.
        </p>
      </statement>
    </definition>
    
    
    <definition xml:id="d_diffeq">
        <title>First-order differential equation</title>
        <statement>
          <p>
            A <term>first-order differential equation</term> for the function <m>f</m>
            is an equation that can be written in the form
            <men xml:id="eq_diffeq">
              f'(x)=F(x,f(x)) 
            </men>
            where <m>F(x,f(x))</m> denotes an arbitrary expression involving <m>x</m> and <m>f(x)</m>.
          </p>
          <p>
            A <term>solution</term> to a differential equation is any function <m>f</m> that satisfies equation <xref ref="eq_diffeq"/>; as such it is useful to think of the function <m>f</m> in this context as an unknown that we are trying to solve for. 
            The <term>general solution</term> to a differential equation is a formula,
            possibly containing undetermined constants,
            describing all solutions to the differential equation.
          </p>
        </statement>
      </definition>
      <definition xml:id="d_sep_diffeq">
        <title>Separable first-order differential equation</title>
        <statement>
          <p>
            A <term>separable differential equation</term> for the function <m>f</m>
            is a differential equation that can be written in the form
            <men xml:id="eq_sep_diffeq_prime">
              f'(x)=g(x)h(f(x))
            </men>,
            or equivalently, letting <m>y=f(x)</m>, 
            <men xml:id="eq_sep_diffeq_alg">
              \frac{dy}{dx}=g(x)h(y)
            </men>.
          </p>
        </statement>
      </definition>

      <algorithm xml:id="proc_sep_vars">
        <title>Separation of variables (algebraic form)</title>
        <statement>
          <p>
            To solve a separable differential equation of the form
            <men xml:id="eq_sep_vars">
              \frac{dy}{dx}=g(x)h(y)
            </men>
            for the function <m>y=f(x)</m>, proceed as follows. 
            <ol>
              <li>
                <title>Separation</title>
                <p>
                  Write the equation as
                  <me>
                    \frac{1}{h(y)}\, dy=g(x)\, dx
                  </me>
                  and take take the indefinite integral of both sides.
                  <me>
                    \int \frac{1}{h(y)}\, dy=\int g(x)\, dx
                  </me>.
                </p>
              </li>
              <li>
                <title>Integration</title>
                <p>
                  Attempt to find an antiderivative <m>F(y)</m> of <m>1/h(y)</m> and an antiderivative <m>G(x)</m> for <m>g(x)</m>.
                </p>
              </li>
              <li>
                <title>Algebra</title>
                <p>
                  The resulting general equation 
                  <men xml:id="eq_sep_vars_implicit">
                    F(y)=G(x)+C
                  </men>
                  is said to be an <term>implicit solution</term> of the differential equation <xref ref="eq_sep_vars"/>. An <term>explicit solution</term> is obtained from <xref ref="eq_sep_vars_implicit"/> by solving for <m>y</m> in terms of <m>x</m> and <m>C</m>, if possible.
                </p>
              </li>
            </ol>
          </p>
        </statement>
      </algorithm>


      
    
      <example xml:id="eg_sep_vars">
        <title>Separation of variables</title>
        <statement>
          <p>
            Solve the following differential equations using separation of variables.
            If an initial condition is given,
            provide the corresponding particular solution.
            Otherwise, give the general solution.
            <ol>
              <li>
                <p>
                  <m>\displaystyle f'(x)=xf(x)+x</m>
                </p>
              </li>
              <li>
                <p>
                  <m>\displaystyle\frac{dy}{dx}=\frac{x^3}{y^2}</m>
                </p>
              </li>
              <li>
                <p>
                  <m>\cot x \cdot f'(x)+f(x)=2</m>, <m>f(0)=0</m>.
                </p>
              </li>
            </ol>
          </p>
        </statement>
        <solution>
          <p>
            <ol>
              <li>
                <p>
                  Let <m>y=f(x)</m>. Following <xref ref="proc_sep_vars"/> we compute 
                  <md>
                    <mrow>\frac{dy}{dx} \amp = x(y+1)</mrow>
                    <mrow>\frac{dy}{y+1} \amp = x\, dx</mrow>
                    <mrow>\int \frac{1}{y+1}\, dy \amp = \int x\, dx</mrow>
                    <mrow> \ln\vert y+1\vert \amp =\frac{1}{2}x^2+C</mrow>
                    <mrow>\vert y+1\vert \amp = e^{x^2/2+C}</mrow>
                    <mrow>y+1\amp =\pm e^{x^2/2}e^C   </mrow>
                    <mrow>y \amp = (\pm e^C)e^{x^2/2}-1</mrow>
                  </md>. 
                  We conclude that 
                  <me>
                    f(x)=De^{x^2/2}-1
                  </me>
                  is the general solution, where <m>D=(\pm e^C)</m>. 
                  How arbitrary is <m>D</m>? Since <m>C</m> was arbitrary, the expression <m>\pm e^C</m> can assume any value except 0. Setting <m>D=0</m> in our formula yields the function <m>f(x)=-1</m>, which by inspection also satisfies the differential equation. We conclude that the general solution is <m>f(x)=De^{x^2/2}-1</m> where <m>D</m> is any real number. 
                </p>
              </li>
              <li>
                <p>
                  Following <xref ref="proc_sep_vars"/> we compute 
                  <md>
                    <mrow> \int y^2\, dy\amp = \int x^3\, dx </mrow>
                    <mrow>\frac{1}{3}y^3 \amp = \frac{1}{4}x^4+C</mrow>
                    <mrow>y^3 \amp = \frac{3}{4}x^4+3C</mrow>
                    <mrow>y \amp = \sqrt[3]{\frac{3}{4}x^4+D}</mrow>
                  </md>
                  where <m>D</m> is any real number. 
                </p>
              </li>
              <li>
                <p>
                  Let <m>y=f(x)</m>. Following <xref ref="proc_sep_vars"/> we compute
                  <md>
                    <mrow>\cot x\cdot \frac{dy}{dx}\amp =2-y  </mrow>
                    <mrow>\frac{dy}{2-y} \amp= \tan x\, dx </mrow>
                    <mrow>\int \frac{1}{2-y}\, dy \amp = \int \tan x\, dx</mrow>
                    <mrow>-\ln\vert 2-y\vert \amp = -\ln\vert \cos x\vert+C </mrow>
                    <mrow>\ln\vert 2-y\vert \amp = \ln\vert \cos x\vert-C </mrow>
                    <mrow>\vert 2-f(x)\vert \amp = e^{\ln\vert \cos x\vert}\, e^{-C}=\vert \cos x\vert e^{-C} </mrow>
                    <mrow>f(x) \amp = 2-D\cos x </mrow>
                  </md>. 
                  Lastly, using the initial condition, we see that 
                  <md>
                    <mrow>f(0)=0 \amp \implies 2-D=0</mrow>
                    <mrow> \amp \implies D=2</mrow>.
                  </md>
                  Thus <m>f(x)=2-2\cos x</m>.
                </p>
              </li>
            </ol>
          </p>
        </solution>
      </example>
      <example xml:id="eg_Newton_cooling">
        <title>Newton's law of cooling</title>
        <statement>
          <p>
            Suppose a hot object cools in a room kept at constant temperature of <m>T_0</m>
            (in celcius).
            Newton's law of cooling states that the rate at which the object cools
            (with respect to time)
            is proportional to the <em>difference</em>
            between its current temperature and the room temperature <m>T_0</m>.
            <ol>
              <li>
                <p>
                  Write a differential equation that describes Newton's law of cooling in this setting.
                </p>
              </li>
              <li>
                <p>
                  Find the general solution to this differential equation.
                </p>
              </li>
              <li>
                <p>
                  Find a the particular solution to the situation where <m>T_0=15
                    ^\circ</m>C, the object's initial temperature is <m>100
                  ^\circ</m>C, and after <m>5</m> minutes the object's temperature is <m>80</m><m>^\circ</m>C.
                </p>
              </li>
            </ol>
          </p>
        </statement>
        <solution>
          <p>
            <ol>
              <li>
                <p>
                  Let temperature <m>T</m> be given by the function <m>T=f(t)</m>. The rate of change of <m>T</m> with respect to <m>t</m> is then <m>f'(t)</m>. Newton's law says this rate of change is proportional to the difference <m>f(t)-T_0</m> of the current temperature of the object and the room temperature.  Mathematically, we write this  proportionality relation as 
                  <men xml:id="eq_Newtons_law">
                    f'(t)=k(f(t)-T_0)
                   </men>,
                  where <m>k</m> is some fixed constant, called the <em>constant of proportionality</em>.
                </p>
              </li>
              <li>
                <p>
                  Equation <xref ref="eq_Newtons_law"/> can be solved using <xref ref="proc_sep_vars"/> in much the same manner as <xref ref="eg_sep_vars"/>, yielding a general solution of the form 
                  <me>
                    f(t)=De^{kt}+T_0
                  </me>,
                  where <m>D</m> is any real number. 
                </p>
              </li>
              <li>
                <p>
                  Assuming <m>T_0=15</m>, we have <m>f(t)=De^{kt}+15</m>. We use the two additional pieces of information to determine the undetermined constants <m>D</m> and <m>k</m>. We have 
                  <md>
                    <mrow>f(0)=100 \amp \implies De^0+15=100\implies D=85</mrow>
                    <mrow>f(5)=80 \amp \implies 85e^{k5}+15=80</mrow>
                    <mrow> \amp \implies e^{k5}=\frac{65}{85}=\frac{13}{17}</mrow>
                    <mrow> \amp\implies 5k=\ln(13/17) </mrow>
                    <mrow>k \amp =\frac{1}{5}\ln (13/17)</mrow>
                  </md>.
                  We conclude that <m>f(t)=85e^{kt}+15</m>, where <m>k=\frac{1}{5}\ln (13/17)</m>. Below you find a graph of <m>f</m> along with its horizontal asymptote <m>y=15</m>. 
                </p>
                <image xml:id="im_Netwons_law" width="50%">
                  <description>Graph of solution to Newton's law</description>
                  <sageplot>
                    x,t=var('x t')
P=plot(85*e^(t*log(13/17)/5)+15, 0,50, color="blue", thickness=2, ticks=[list(range(0,60,10)),list(range(0,110,10))])
Q=plot(15,x,0,50, color="green", thickness=2)
P+Q
                  </sageplot> 
                </image>
              </li>
            </ol>
          </p>
        </solution>
      </example>
      
</section>