<?xml version="1.0" encoding="UTF-8"?>

<section xml:id="s_substitution" xmlns:xi="http://www.w3.org/2001/XInclude">
    <title>Substitution</title>
<p>
    In the spirit of the De Morgan quote in <xref ref="mantra_integration_differentiation"/>, running various derivative rules in reverse yields different integration techniques. The <xref ref="th_subst" text="custom">substitution theorem</xref> is nothing more than the chain rule expressed in terms of antiderivatives. 
</p>
<theorem xml:id="th_subst">
    <title>Substitution</title>
    <statement>
      <p>
        Let <m>u=g(x)</m> be a differentiable function on its domain,
        and suppose <m>f</m> is continuous on the range of <m>g</m>.
        If <m>F(x)</m> is an antiderivative of <m>f(x)</m>, 
        then <m>F(g(x))</m> is an antiderivative of <m>f(g(x))g'(x)</m>: <ie/>, 
        <men xml:id="eq_substitution">
          \int f(g(x))g'(x)\, dx=F(g(x))+C
        </men>.
      </p>
    </statement>
    <proof>
        <p>
            Assume <m>F</m> is an antiderivative of <m>f</m>, so that <m>F'(x)=f(x)</m> for all <m>x</m> in the domain of <m>f</m>. It follows that 
            <md>
                <mrow>\frac{d}{dx}F(g(x)) \amp =F'(g(x))g'(x)\amp \text{(chain rule)}</mrow>
                <mrow> \amp = f(g(x))g'(x) \amp (F'=f) </mrow>
            </md>.
        </p>
    </proof>
  </theorem>
  <example xml:id="eg_subst_easy">
    <title>Substitution:straightforward</title>
    <statement>
        <p>
            Use the substitution technique to compute the following indefinite integrals.
            <ol>
                <li>
                    <p>
                      <m>\displaystyle\int -\sin t\, \sqrt{\cos t}\, dt</m>
                    </p>
                  </li>
                  <li>
                    <p>
                      <m>\displaystyle\int \frac{\sin(\sqrt{s})}{2\sqrt{s}}\, ds</m>
                    </p>
                  </li>
                  <li>
                <p>
                  <m>\displaystyle\int x^2\sqrt{x^3+1}\, dx</m>
                </p>
              </li>
            </ol>
        </p>
    </statement>
    <solution>
        <p>
            <ol>
              <li>
                <p>
                  We have  <m> -\sin t\, \sqrt{\cos t}=f(g(t))g'(t)</m> where <m>f(t)=\sqrt{t}</m> and <m>g(t)=\cos t</m>. Since <m>F(t)=\frac{2}{3}\sqrt{x}</m> is an antiderivative of <m>f</m>, <xref ref="th_subst"/> tells us that <m>F(g(t))=\frac{2}{3}(\cos t)^{3/2}</m> is an antiderivative of <m>f(g(x))g'(x)= -\sin t\, \sqrt{\cos t}</m>. We conclude 
                  <me>
                    \int  -\sin t\, \sqrt{\cos t}\, dt =\frac{2}{3}(\cos t)^{3/2}+C
                  </me>.
                </p>
              </li>
              <li>
                <p>
                  We have  <m> \frac{\sin(\sqrt{s})}{2\sqrt{s}}=f(g(s))g'(s)</m> where <m>f(s)=\sqrt{s}</m> and <m>g(s)=\sqrt{s}</m>. Since <m>F(s)=-\cos t</m> is an antiderivative of <m>f</m>, <xref ref="th_subst"/> tells us that <m>F(g(s))=-\cos(\sqrt{s})</m> is an antiderivative of <m>f(g(x))g'(x)= \frac{\sin(\sqrt{s})}{2\sqrt{s}}</m>. We conclude 
                  <me>
                    \int  \frac{\sin(\sqrt{s})}{2\sqrt{s}}\, ds =-\cos(\sqrt{s})+C
                  </me>.
                </p>
              </li>
              <li>
                <p>
                  A similar approach as above can be applied, though here we have <m>x^2\sqrt{x^3+1}=\frac{1}{3}f(g(x))g'(x)</m>, where <m>f(x)=\sqrt{x}</m> and <m>g(x)=x^3+1</m>. It follows that 
                  <me>
                    \int x^2\sqrt{x^3+1}\, dx=\frac{1}{3}\int f(g(x))g'(x)\, dx=\frac{2}{9}(x^3+1)^{3/2}+C
                  </me>,
                  since <m>F(x)=\frac{2}{3}x^{3/2}</m> is an antiderivative of <m>f(x)=\sqrt{x}</m>. 
                  
                </p>
              </li>
            </ol>
        </p>
    </solution>
  </example>
  <p>
    The usefulness of <xref ref="th_subst"/> depends on your ability to express the given integrand in the very particular form <m>f(g(x))g'(x)</m>. This is not always as easy to do as it was in <xref ref="eg_subst_easy"/>. The <xref ref="proc_sub" text="custom">substitution procedure</xref> facilitates this process, giving it a more algebraic flavor. 
  </p>
  <algorithm xml:id="proc_sub">
    <title>Substitution</title>
    <statement>
        <p>
           To compute an indefinite integral <m>\int f(x)\, dx</m> using substitution, proceed as follows. 
           <ol>
            <li>
                <title>Choose substitution</title>
                <p>
                    Choose a differentiable function <m>u=g(x)</m> and write down the two substitution equations 
                    <mdn>
                        <mrow xml:id="eq_u">u \amp =g(x)</mrow>
                        <mrow xml:id="eq_du">du \amp = g'(x)dx</mrow>
                    </mdn>.
                </p>
            </li>
            <li>
                <title>Transform</title>
                <p>
                    Use <xref first="eq_u" last="eq_du"/> and algebra to transform the indefinite integral <m>\int f(x)\, dx</m> into a new indefinite integral <m>\int h(u)\, du</m> expressed entirely in terms of <m>u</m>.  
                </p>
            </li>
            <li>
                <title>Compute and substitute</title>
                <p>
                    Compute <m>\int h(u)\, du=F(u)+C</m>, if possible. Substitute <m>u=g(x)</m> for <m>u</m> to conclude that 
                    <md>
                        <mrow>\int f(x)\, dx \amp =\int h(u)\, du</mrow>
                        <mrow> \amp = F(u)+C</mrow>
                        <mrow> \amp = F(g(x))+C</mrow>
                    </md>.
                </p>
            </li>
           </ol>  
        </p>
    </statement>
  </algorithm>
  <remark>
    <title>Substitution procedure</title>
    <p>
        <xref ref="proc_sub"/> is so algebraic in flavor that we sometimes forget that the chain rule is in play here! It is baked into the transformation step 
        <me>
            \int f(x)\, dx=\int h(u)\, du
        </me>. 
        Using the substitution equations <xref first="eq_u" last="eq_du"/>, we see that this equality is really just an algebraic short hand for the equality 
        <me>
            \int f(x)\, dx= \int h(g(x))g'(x)\,dx
        </me>.
        Now the <xref ref="th_subst" text="custom">substitution theorem</xref> tells us that if <m>F</m> is an antiderivative of <m>h</m>, then <m>F(g(x))</m> is an antiderivative of <m>h(g(x))g'(x)</m>. This is why our conclusion 
        <me>
            \int f(x)\, dx=F(g(x))+C
        </me>
        is valid. 
    </p>
  </remark>
  <example xml:id="eg_subst_hard">
    <title>Substitution: less straightforward</title>
    <statement>
        <p>
            Use the substitution technique to compute the following indefinite integrals.
            <ol>
              <li>
                <p>
                  <m>\displaystyle\int\frac{x}{\sqrt{x+1}}\, dx</m>
                </p>
              </li>
              <li>
                <p>
                  <m>\displaystyle\int (1+\sqrt{t})^{100}\, dt</m>
                </p>
              </li>
            </ol>
        </p>
    </statement>
    <solution>
        <p>
            <ol>
              <li>
                <p>
                  We choose the substitution 
                  <mdn >
                    <mrow xml:id="eq_subst1_u"> u \amp= x+1 </mrow>
                    <mrow xml:id="eq_subst1_du">du \amp = dx </mrow>
                  </mdn>
                  Equation <xref ref="eq_subst1_u"/> implies <m>x=u-1</m>. Transforming the integral, we get 
                  <md>
                    <mrow> \int\frac{x}{\sqrt{x+1}}\, dx\amp = \int \frac{u-1}{\sqrt{u}}\, du </mrow>
                    <mrow> \amp = \int u^{1/2}-u^{-1/2}\, du</mrow>
                    <mrow> \amp = \frac{2}{3}u^{3/2}-2u^{1/2}+C</mrow>
                    <mrow> \amp = \frac{2}{3}(x+1)^{3/2}-2(x+1)^{1/2}+C</mrow>
                  </md>. 
                </p>
              </li>
              <li>
                <p>
                  We choose the substitution 
                  <mdn >
                    <mrow xml:id="eq_subst2_u"> u \amp= 1+\sqrt{t} </mrow>
                    <mrow xml:id="eq_subst2_du">du \amp = \frac{1}{2\sqrt{t}} dt </mrow>
                  </mdn>
                  Equation <xref ref="eq_subst2_du"/> implies <m>dt=2\sqrt{t}du</m>. By <xref ref="eq_subst2_du"/>, we have <m>\sqrt{t}=u-1</m>. Thus  <m>dt=2\sqrt{t}du=2(u-1)</m>. Transforming the integral, we get 
                  <md>
                    <mrow> \int(1+\sqrt{t})^{100}\, dt \amp = \int u^{100}2(u-1)\, du </mrow>
                    <mrow> \amp = 2\int u^{101}-u^{100} du</mrow>
                    <mrow> \amp = \frac{2}{102}u^{102}-\frac{2}{101}u^{101}+C</mrow>
                    <mrow> \amp = \frac{2}{102}(1+\sqrt{t})^{102}-\frac{2}{101}(1+\sqrt{t})^{101}+C</mrow>
                  </md>. 
                </p>
              </li>
            </ol>
        </p>
    </solution>
  </example>
  <p>
    <xref ref="proc_sub"/> is a technique for computing antiderivatives. Of course, we can combine this with <xref ref="th_FTC_II" text="title"/> to obtain a substitution method for definite integrals. In the next section we will provide an alternative, more streamlined approach to computing definite integrals using substitution. 
  </p>
  <algorithm xml:id="proc_sub_2step">
    <title>Definite integral substitution: 2-step</title>
    <statement>
        <p>
            To compute a definite integral <m>\int_a^b f(x)\, dx</m> using substitution, proceed as follows. 
            <ol>
                <li>
                    <p>
                        Find an antiderivative <m>F</m> of <m>f</m> using a substitution <m>u=g(x)</m> and <xref ref="proc_sub"/>. 
                    </p>
                </li>
                <li>
                    <p>
                        Use <xref ref="th_FTC_II" text="title"/> to conclude that 
                        <me>
                            \int_a^b f(x)\, dx=F(b)-F(a)
                        </me>.                        
                    </p>
                </li>
            </ol>
        </p>
    </statement>
  </algorithm>
  <example>
    <title>Definite integral substitution: 2-step technique</title>
    <statement>
        <p>
            Use substitution to compute <m>\displaystyle\int_1^2\frac{x}{\sqrt{x+1}}\, dx</m>. 
        </p>
    </statement>
    <solution>
        <p>
            We saw in <xref ref="eg_subst_hard"/> that an antiderivative of the given integrand is <me>F(x)=\frac{2}{3}(x+1)^{3/2}-2(x+1)^{1/2}=2(x+1)^{1/2}\left(\frac{1}{3}x-\frac{2}{3}\right)</me>. We conclude using <xref ref="th_FTC_II" text="title"/> that 
            <md>
              <mrow>\int_1^2\frac{x}{\sqrt{x+1}}\, dx \amp =F(2)-F(1)</mrow>
              <mrow> \amp = 2(3)^{1/2}\left(\frac{2}{3}-\frac{2}{3}\right)-2(2)^{1/2}\left(\frac{1}{3}-\frac{2}{3}\right)</mrow>
              <mrow> \amp = \frac{2\sqrt{2}}{3}</mrow>
            </md>.
        </p>
    </solution>
  </example>

</section>