<?xml version="1.0" encoding="UTF-8"?>

<section xml:id="s_trig_subst" xmlns:xi="http://www.w3.org/2001/XInclude">
    <title>Trigonometric substitution</title>
<p>
    Trigonometric substitution is an example of a more general integral technique that we call <em>inverse substitution</em>. In turn, inverse substitution is really just an application of the substitution where our substitution function is <em>invertible</em>. 
</p>
    
<algorithm xml:id="proc_inv_sub_indef">
    <title> Inverse substitution: indefinite integral</title>
      <statement>
        <p>
          To compute <m>\displaystyle\int f(x)\, dx</m> using inverse substitution,
          proceed as follows.
          <ol>
            <li>
              <p>
                Choose a one-to-one, differentiable substitution function <m>g</m> with differentiable inverse and assemble the two equations
                <md>
                  <mrow>x\amp =g(t)</mrow>
                  <mrow>dx\amp =g'(t)\, dt</mrow>
                </md>
              </p>
            </li>
            <li>
              <p>
                Compute
                <me>
                  \int f(g(t))g'(t)\, dt=F(t)+C
                </me>.
              </p>
            </li>
            <li>
              <p>
                Conclude that
                <me>
                  \int f(x)\, dx=F(g^{-1}(x))+C
                </me>.
                When an explicit formula for <m>g^{-1}(x)</m> is not available, we attempt to compute <m>F(g^{-1}(x))</m> by rewriting <m>F(t)</m> in terms of <m>x</m> using the equation <m>x=g(t)</m>.
              </p>
            </li>
          </ol>
        </p>
      </statement>
</algorithm>


<algorithm xml:id="proc_trig_sub">
  <title>Trigonometric substitution</title>
  <statement>
    <p>
      The table below indicates potentially helpful inverse substitutions for functions <m>f</m> of various types. 
      <md>
        <mrow>f(x) \text{ contains }  \sqrt{a^2-x^2}\amp \implies    \begin{array}{rcl} x\amp =\amp a\sin\theta \\ dx\amp = \amp a\cos\theta\, d\theta \end{array} \hspace{5pt} \text{ where } \theta\in [-\pi/2, \pi/2]</mrow>
        <mrow> \amp </mrow>
        <mrow>f(x) \text{ contains } \hspace{10pt}  x^2+a^2 \amp \implies    \begin{array}{rcl} x\amp =\amp a\tan\theta \\ dx\amp = \amp a\sec^2\theta\, d\theta \end{array} \hspace{5pt} \text{ where } \theta\in (-\pi/2, \pi/2)</mrow>
        <mrow> \amp </mrow>
        <mrow>f(x) \text{ contains }  \sqrt{x^2-a^2} \amp \implies    \begin{array}{rcl} x\amp =\amp a\sec\theta \\ dx\amp = \amp a\sec \theta\tan\theta \, d\theta \end{array} \hspace{5pt} \text{ where } \theta\in [0,\pi/2)\cup (\pi/2, \pi]</mrow>
      </md>.
    </p>
  </statement>
</algorithm>

<algorithm xml:id="proc_ref_triangles">
  <title>Reference triangles</title>
  <statement>
    <p>
      When finishing an integral computation <m>\int f(x)\, dx</m> using an trigonometric substitution, the following types of <term>reference triangles</term> are useful for converting your expression back in terms of <m>x</m>. 
    </p>
    <p>
      For the sake of space, we only provide examples of reference triangles where the angle <m>\theta</m> lies in <m>[0,\pi/2]</m>. In practice, you should provide a reference triangle diagram that reflects the interval <m>\theta</m> is restricted to, and take care with the sign of the various trigonometric values.  
    </p>
      <ol>
        <li>
          <p>
            Consider the substitution <m>x=a\sin \theta</m>, where <m>a</m> is positive. A reference diagram like the following helps us see that 
            <md>
              <mrow>\cos\theta \amp = \frac{\sqrt{a^2-x^2}}{a} \amp \tan\theta\amp = \frac{x}{a}</mrow>
            </md>.  
          </p>
          <figure xml:id="fig_sin_ref_tri">
            <caption>Reference triangle for <m>x=a\sin\theta</m></caption>
            <image xml:id="im_sin_ref_tri" width="50%">
              <description>Reference triange for sine substitution</description>
              <sageplot>
                T=line([(0,0),(1/2,1/2),(1/2,0),(0,0)], axes=False, ticks=[[],[]],aspect_ratio=1.1)
                t1=text(r'$x=a\sin\theta$', (.58,1/4), fontsize=16, color="black")
                t2=text(r'$\sqrt{a^2-x^2}$', (.3,1/32), fontsize=16, color="black")
                t3=text("$a$", (1/4,.3),fontsize=16,color="black")
                t4=text(r"$\theta$", (2/32, .02),fontsize=16, color="black")
                T+t1+t2+t3+t4
              </sageplot>
            </image>
          </figure>
        </li>
        <li>
          <p>
            Consider the substitution <m>x=a\tan \theta</m>, where <m>a</m> is positive. A reference diagram like the following allows us to deduce that 
            <md>
              <mrow>\cos\theta \amp = \frac{a}{\sqrt{x^2+a^2}} \amp \sin\theta\amp =\frac{x}{\sqrt{x^2+a^2}}</mrow>
            </md>.
          </p>
            <figure xml:id="fig_tan_ref_tri">
              <caption>Reference triangle for <m>x=a\tan\theta</m></caption>
              <image xml:id="im_tan_ref_tri" width="50%">
                <description>Reference triangle for tangent substitution</description>
                <sageplot>
                  T=line([(0,0),(1/2,1/2),(1/2,0),(0,0)], axes=False, ticks=[[],[]],aspect_ratio=1.1)
                  t1=text(r'$x=a\tan\theta$', (.58,1/4), fontsize=16, color="black")
                  t2=text(r'$a$', (.3,1/32), fontsize=16, color="black")
                  t3=text(r"$\sqrt{a^2+x^2}$", (3/16,.3),fontsize=16,color="black")
                  t4=text(r"$\theta$", (2/32, .02),fontsize=16, color="black")
                  T+t1+t2+t3+t4
                </sageplot>
              </image>
            </figure>
        </li>
        <li>
          <p>
            Consider the substitution <m>x=a\sec \theta</m>, where <m>a</m> is positive. A reference diagram like the following allows us to deduce that 
            <md>
              <mrow> \sin \theta\amp =\frac{\sqrt{a^2-x^2}}{\abs{x}} \amp \tan \theta\amp =\begin{cases} 
                \frac{\sqrt{x^2-a^2}}{a} \amp \text{if } \theta\in [0,\pi/2) \\
                -\frac{\sqrt{x^2-a^2}}{a} \amp \text{if } \theta\in (\pi/2, \pi].
                \end{cases}
              </mrow>
            </md>
          </p>
          <figure xml:id="fig_sec_ref_tri">
            <caption>Reference triangle for <m>x=a\sec\theta</m></caption>
            <image xml:id="im_sec_ref_tri" width="50%">
              <description>Reference triangle for secant substitution</description>
              <sageplot>
                T=line([(0,0),(1/2,1/2),(1/2,0),(0,0)],axes=False, ticks=[[],[]],aspect_ratio=1.1)
                t1=text(r'$\sqrt{x^2-a^2}$', (.575,1/4), fontsize=16, color="black")
                t2=text(r'$a$', (.3,1/32), fontsize=16, color="black")
                t3=text(r"$x=a\sec\theta$", (.2,.3),fontsize=16,color="black")
                t4=text(r"$\theta$", (2/32, .02),fontsize=16, color="black")
                T+t1+t2+t3+t4
              </sageplot>
            </image>
          </figure>  
        </li>
      </ol>
  </statement>
</algorithm>

<algorithm xml:id="proc_inv_sub_def">
    <title>Inverse substitution: definite integral</title>
      <statement>
        <p>
          To compute <m>\displaystyle\int_a^b f(x)\, dx</m> using inverse substitution,
          proceed as follows. 
          <ol>
            <li>
              <p>
                Choose a one-to-one, differentiable substitution function <m>g</m> with differentiable inverse and write down the two inverse substitution equations
                <md>
                  <mrow>x\amp =g(t)</mrow>
                  <mrow>dx\amp =g'(t)\, dt</mrow>
                </md>
              </p>
            </li>
            <li>
              <p>
                Conclude that 
                <me>
                  \displaystyle\int_{x=a}^{x=b} f(x)\, dx=\int_{t=g^{-1}(a)}^{t=g^{-1}(b)}f(g(t))g'(t)\, dt
                </me>.
              </p>
            </li>
          </ol>
        </p>
      </statement>
</algorithm>
<example xml:id="eg_sin_sub">
  <title>Sine substitution</title>
  <statement>
    <p>
      <p>
        Find an antiderivative of <m>f(x)=\sqrt{1-x^2}</m>.
      </p>
    </p>
  </statement>
  <solution>
    <p>
      Using <xref ref="proc_trig_sub"/> we try the inverse substitution <m>x=\sin \theta, dx=\cos \theta\, d\theta</m> with restriction <m>-\pi/2\leq \theta\leq \pi/2</m>. We compute 
      <md>
        <mrow>\int \sqrt{1-x^2}\, dx \amp = \int \sqrt{1-\sin^2\theta}\,  \cos\theta\, d\theta</mrow>
        <mrow> \amp = \int \sqrt{\cos^2\theta} \, \cos\theta\, d\ theta</mrow>
        <mrow> \amp = \int \abs{\cos \theta}\cos \theta\, d\theta</mrow>
        <mrow> \amp = \int \cos^2\theta\, d\theta \amp (\theta\in [-\pi/2,\pi/2]\implies \cos \theta\geq 0)</mrow>
        <mrow> \amp = \frac{1}{2}\theta+\frac{1}{4}\sin(2\theta) +C</mrow>
        <mrow> \amp = \frac{1}{2}\theta+\frac{1}{2}\sin\theta\cos\theta +C</mrow>
        <mrow> \amp = \frac{1}{2}\arcsin(x)+\frac{1}{2}\sin(\arcsin(x))\cos(\arcsin x)+C</mrow>
        <mrow> \amp = \frac{1}{2}\arcsin x+ \frac{1}{2}x\sqrt{1-x^2}+C</mrow>
      </md>.
      Here we have used once again that <m>\cos(\arcsin x)=\sqrt{1-x^2}</m>. Recall that this can be derived using the following reference triangle. 
      <image xml:id="im_ref_tri_1" width="75%">
        <description>Reference triangle for <m>x=\sin\theta</m></description>
        <sageplot>
  T=line([(0,0),(1/2,1/2),(1/2,0),(0,0)], axes=False, ticks=[[],[]],aspect_ratio=1.1)
  t1=text(r'$x=\sin\theta$', (.58,1/4), fontsize=16, color="black")
  t2=text(r'$\sqrt{1-x^2}=\cos\theta$', (.3,1/32), fontsize=16, color="black")
  t3=text("$1$", (1/4,.3),fontsize=16,color="black")
  t4=text(r"$\theta$", (2/32, .02),fontsize=16, color="black")
  T+t1+t2+t3+t4
        </sageplot>
      </image>
    </p>
    
  </solution>
</example>
<example xml:id="eg_area_circle">
  <title>Area of circle</title>
  <statement>
    <p>
      Derive the area formula for a circle of radius <m>r</m>. 
    </p>
  </statement>
  <solution>
    <p>
      Let <m>\mathcal{C}</m> be a circle of radius <m>r</m>. Choosing the origin to be the center of <m>\mathcal{C}</m>, we may assume that <m>\mathcal{C}</m> has equation <m>x^2+y^2=r^2</m>. The interior of the circle is the region <m>\mathcal{R}</m> lying between the graphs of the two function <m>y=f(x)=+\sqrt{r^2-x^2}</m> and <m>y=g(x)=-\sqrt{r_2-x^2}</m> from <m>x=-r</m> to <m>x=r</m>. Using <xref ref="d_area_between_curves_x"/> we compute
      <md>
        <mrow>\operatorname{area}\mathcal{R} \amp = \int_{-r}^r\sqrt{r^2-x^2}-(-\sqrt{r^2-x^2}) \, dx </mrow>
        <mrow> \amp = 2\int_{-r}^{r}\sqrt{r^2-x^2}\, dx</mrow>
        <mrow> \amp = 2\int_{-\pi/2}^{\pi/2}\sqrt{r^2-r^2\sin^2\theta }\, r\cos \theta\, d\theta \amp (x=r\sin\theta, dx=r\cos\theta dx)</mrow>
        <mrow> \amp 2r^2\int_{-\pi/2}^{\pi/2}\sqrt{\cos^2\theta}\cos\theta\, d\theta</mrow>
        <mrow> \amp 2r^2\int_{-\pi/2}^{\pi/2}\abs{\cos\theta}\cos\theta\, d\theta</mrow>
        <mrow> \amp = 2r^2\int_{-\pi/2}^{\pi/2}\cos^2\theta\, d\theta \amp (\theta\in [-\pi/2,\pi/2]\implies \cos\theta &gt; 0)
        </mrow>
        <mrow> \amp = 2r^2(\frac{1}{2}\theta+\frac{1}{2}\sin 2\theta)\Bigr\vert_{-\pi/2}^{\pi/2} \amp (\cos^2\theta=\frac{1}{2}(1+\cos 2\theta))</mrow>
        <mrow> \amp = 2r^2(\pi/4-(-\pi/4))</mrow>
        <mrow> \amp = \pi r^2</mrow>
      </md>.
    </p>
  </solution>
</example>
<example xml:id="eg_tan_sub">
  <title>Tangent substitution</title>
  <statement>
    <p>
      Compute <m>\displaystyle\int \frac{1}{x^2\sqrt{x^2+4}}\, dx</m>.
    </p>
  </statement>
  <solution>
    <p>
      Following <xref ref="proc_trig_sub"/>, we try the inverse substitution <m>x=2\tan\theta</m>, <m>dx=2\sec^2\theta dx</m>, <m>\theta\in (-\pi/2, \pi/2)</m>: 
      <md>
        <mrow> \int \frac{1}{x^2\sqrt{x^2+4}}\, dx \amp = \int \frac{1}{4\tan^2 \theta\sqrt{4\tan^2\theta+4}}\cdot 2\sec^2\theta\, d\theta </mrow>
        <mrow> \amp = \frac{1}{4}\int \frac{1}{\tan^2\theta\sqrt{\sec^2\theta}}\cdot \sec^2\theta\, d\theta</mrow>
        <mrow> \amp = \frac{1}{4}\int \frac{1}{\tan^2\theta\abs{\sec\theta}}\cdot \sec^2\theta\, d\theta</mrow>
        <mrow> \amp =\frac{1}{4}\int \frac{1}{\tan^2\theta \sec\theta}\cdot \sec^2\theta\, d\theta \amp (\theta\in (-\pi/2, \pi/2)\implies \sec\theta &gt; 0)</mrow>
        <mrow> \amp =\frac{1}{4}\int \frac{\sec\theta}{\tan^2\theta}\, d\theta</mrow>
        <mrow> \amp = \frac{1}{4}\int \frac{\cos \theta}{\sin^2\theta}\, d\theta</mrow>
        <mrow> \amp = -\frac{1}{4\sin\theta}+C</mrow>
        <mrow> \amp = -\frac{\sqrt{x^2+4}}{4x}+C</mrow>
      </md>.
      Here we deduce that <m>\sin\theta=\frac{x}{\sqrt{x^2+4}}</m> from the reference triangle for <m>x=2\tan\theta</m>.
      <image xml:id="im_tan_ref_tri_eg" width="50%">
        <description>Reference triangle for tangent substitution</description>
        <sageplot>
          T=line([(0,0),(1/2,1/2),(1/2,0),(0,0)], axes=False, ticks=[[],[]],aspect_ratio=1.1)
          t1=text(r'$x=2\tan\theta$', (.58,1/4), fontsize=16, color="black")
          t2=text(r'$2$', (.3,1/32), fontsize=16, color="black")
          t3=text(r"$\sqrt{x^2+4}$", (3/16,.3),fontsize=16,color="black")
          t4=text(r"$\theta$", (2/32, .02),fontsize=16, color="black")
          T+t1+t2+t3+t4
        </sageplot>
      </image>


    </p>
  </solution>
</example>
<example xml:id="eg_sec_sub_easy">
  <title>Secant substitution</title>
  <statement>
    <p>
      Let <m>a</m> be a fixed positive number. Compute <m>\displaystyle \int \frac{1}{\sqrt{x^2-a^2}}\, dx</m>.
    </p>
  </statement>
  <solution>
    <p>
      Following <xref ref="proc_trig_sub"/> we try the inverse substitution <m>x=a\sec\theta</m>, <m>dx=a\sec\theta\tan\theta</m>, <m>\theta\in [0,\pi/2)\cup (\pi/2, \pi]</m>: 
      <md>
        <mrow> \int \frac{1}{\sqrt{x^2-a^2}}\, dx \amp = \int \frac{1}{\sqrt{a^2\sec^2 x-a^2}}\cdot a\sec\theta\tan\theta\, dx </mrow>
        <mrow> \amp =\int \frac{1}{\sqrt{\tan^2 \theta}}\sec\theta\tan\theta\, d\theta</mrow>
        <mrow> \amp = \begin{cases}
          \int \frac{1}{\tan\theta}\sec\theta\tan\theta\, d\theta \amp \text{if } \theta\in [0,\pi/2) \\
          -\int\frac{1}{\tan\theta}\sec\theta\tan\theta\, d\theta \amp \text{if }\theta\in (\pi/2,\pi]
        \end{cases}
        </mrow>
        <mrow> \amp = 
          \begin{cases}
          \int \sec\theta\, d\theta \amp  \text{if } \theta\in [0,\pi/2) \\
          -\int\sec\theta\, d\theta \amp \text{if }\theta\in (\pi/2,\pi]
          \end{cases}
        </mrow>
        <mrow> \amp = \begin{cases}
          \ln\abs{\sec\theta+\tan\theta}+C \amp  \text{if } \theta\in [0,\pi/2) \\
          -\ln\abs{\sec\theta+\tan\theta}+C \amp \text{if }\theta\in (\pi/2,\pi]
        \end{cases}
         </mrow>
         <mrow> \amp =\begin{cases}
          \ln\abs{\frac{x}{a}+\frac{\sqrt{x^2-a^2}}{a}}+C \amp  \text{if } \theta\in [0,\pi/2) \\
          -\ln\abs{\frac{x}{a}-\frac{\sqrt{x^2-a^2}}{a}}+C \amp \text{if }\theta\in (\pi/2,\pi]
        \end{cases} \amp (<xref ref="fig_sec_ref_tri"/>)</mrow>
        <mrow> \amp =\ln\abs{\frac{x+\sqrt{x^2-a^2}}{a}} \amp (\ln\abs{\frac{x}{a}+\frac{\sqrt{x^2-a^2}}{a}}=-\ln\abs{\frac{x}{a}-\frac{\sqrt{x^2-a^2}}{a}}!)</mrow>
        <mrow> \amp = \ln\abs{x+\sqrt{x^2-a^2}}-\ln a+C</mrow>
        <mrow> \amp = \ln\abs{x+\sqrt{x^2-a^2}}+D</mrow>
      </md>. 

    </p>
  </solution>
</example>
<example xml:id="eg_sec_sub">
  <title>Secant substitution: definite</title>
  <statement>
    <p>
      Compute <m>\displaystyle\int_{-\sqrt{2}}^{-2/\sqrt{3}}\frac{\sqrt{x^2-1}}{x}\, dx</m>.
      </p>
  </statement>
  <solution>
    <p>
      We use the inverse substitution <m>x=\sec\theta, dx=\sec\theta\tan\theta</m>. Solve <m>-1/\sqrt{2}=\sec\theta</m> and <m>-2/\sqrt{3}=\sec\theta</m> for <m>\theta\in [0,\pi/2)\cup (\pi/2,\pi]</m>, we see that the new limits of integration are <m>\theta=3\pi/4</m> and <m>\theta=5\pi/6</m>. Thus we have 
      <md>
        <mrow> \int_{-\sqrt{2}}^{-2/\sqrt{3}}\frac{\sqrt{ \theta^2-1}}{ \theta}\, d \theta \amp = \int_{3\pi/4}^{5\pi/6}\frac{\sqrt{\sec^2 \theta-1}}{\sec  \theta}\cdot \sec  \theta\tan \theta\,  d\theta </mrow>
        <mrow> \amp =\int_{3\pi/4}^{5\pi/6}\frac{\abs{\tan \theta}}{\sec \theta}\cdot \sec \theta\tan \theta\,  d\theta  </mrow>
        <mrow> \amp = \int_{3\pi/4}^{5\pi/6}-\tan^2 \theta\,  d\theta  \amp (\theta\in (\pi/2, \pi]\implies \tan\theta&lt; 0)</mrow>
        <mrow> \amp = \int_{3\pi/4}^{5\pi/6}1-\sec^2 \theta\, d\theta</mrow>
        <mrow> \amp = \theta-\tan\theta\Bigr\vert_{3\pi/4}^{5\pi/6}</mrow>
        <mrow> \amp = \frac{\pi}{12}+\frac{1}{\sqrt{3}}-1</mrow>
      </md>.
    </p>
  </solution>
</example>

<example xml:id="eg_sec_sub_again">
  <title>Secant substitution: indefinite</title>
  <statement>
    <p> Find an antiderivative <m>F</m> of the function  <m>f(x)=\frac{\sqrt{x^2-1}}{x}\, dx</m> on the domain <m>(-\infty,-1]\cup [1,\infty)</m>. The only inverse trigonometric functions allowed to appear in your formula for <m>F</m> are <m>\arcsin x</m> and <m>\arctan x</m>. 
    </p>
  </statement>
  <!-- <hint>
    <p>
      Treat the cases <m>x\geq 1</m> and <m>x\leq -1</m> separately and use the absolute value function to combine your two results into a single formula. 
    </p>
  </hint> -->
  <solution>
    <p>
      To be assigned on written homework. 
    </p>
  </solution>
</example>
</section>