<?xml version="1.0" encoding="UTF-8"?>

<section xml:id="s_trig_int" xmlns:xi="http://www.w3.org/2001/XInclude">
    <title>Trigonometric integrals</title>
    <p>
      We now develop an integration technique for two <em>very particular</em> types of integrals: 
      <md>
        <mrow>\int \sin^m x\cos^n x\, dx \amp \amp \int \tan^m x\sec^n x\, dx </mrow>
      </md>.
      Why these particular pairings of products of functions? In a nutshell, because one of the following four choices of substitution will often come in handy: 
      <md>
        <mrow>u\amp =\sin x \amp u\amp =\tan x </mrow>
        <mrow>du\amp =\cos x\, dx \amp du\amp =\sec^2 x</mrow>
        <mrow> \amp </mrow>
        <mrow>u\amp =\cos x \amp u\amp =\sec x </mrow>
        <mrow>du\amp =-\sin x\, dx \amp du\amp =\sec x\tan x</mrow>
      </md>.
      <xref ref="proc_int_sincos"/> and <xref ref="proc_int_tansec"/> articulate in greater detail when and where such substitutions will be useful. The basic principle is that a given substitution as above will help, when after <q>peeling off</q> part of the integrand to account for the <m>du</m>, the remaining part of the integrand can be expressed completely in terms of <m>u</m>.  
    </p>
    <theorem xml:id="th_trig_identities">
        <title>Trigonometric identities</title>
      <statement>
        <p>
          The following identities hold for all real numbers <m>\theta</m> and <m>\phi</m> for which the given expression is defined.
          <ol>
            <li>
                <title>Pythagorean identities</title>
                <p>
                    <md>
                        <mrow>\sin^2\theta+\cos^2\theta \amp = 1 \amp \tan^2\theta+1\amp = \sec^2\theta </mrow>
                    </md>
                </p>
            </li>
            <li>
                <title>Sum-to-product and double-angle formulas</title>
                <p>
                    <md>
                        <mrow>\sin(\theta+\phi) \amp =\sin\theta\cos\phi+\cos\theta\sin\phi 
                            \amp \sin(\theta-\phi) \amp =\sin\theta\cos\phi-\cos\theta\sin\phi </mrow>
                        <mrow> \cos(\theta+\phi)\amp =\cos\theta\cos\phi-\sin\theta\sin\phi 
                            \amp \cos(\theta-\phi)\amp =\cos\theta\cos\phi+\sin\theta\sin\phi 
                        </mrow>
                        <mrow> \sin(2\theta)\amp =2\sin\theta\cos\theta </mrow>
                        <mrow> \cos(2\theta)  \amp = \cos^2\theta-\sin^2\theta </mrow>
                    </md>.
                </p>
            </li>
           <li>
            <title>Product-to-sum and square formulas</title>
              <p>
                <md>
                    <mrow>\sin\theta\sin\phi \amp = \frac{1}{2}(\cos(\theta-\phi)-\cos(\theta+\phi)) </mrow>
                    <mrow>\cos\theta\cos\phi \amp =\frac{1}{2}(\cos(\theta-\phi)+\cos(\theta+\phi)) </mrow>
                    <mrow> \sin\theta\cos\phi \amp = \frac{1}{2}(\sin(\theta-\phi)+\sin(\theta+\phi))</mrow>
                    <mrow> \sin^2\theta \amp = \frac{1}{2}(1-\cos 2\theta) </mrow>
                    <mrow> \cos^2\theta\amp = \frac{1}{2}(1+\cos 2\theta)</mrow>
                </md>.
              </p>
            </li>
          </ol>
        </p>
      </statement>
    </theorem>
    
    <algorithm xml:id="proc_int_sincos">
        <title>Integrating <m>\sin^m x\cos^n x</m></title>
        <statement>
          <p>
            Let <m>m</m> and <m>n</m> be nonnegative integers.
            When computing
            <me>
              \int \sin^m x\cos^n x\, dx
            </me>
            use the following strategies.
            <ol>
              <li>
                <title>Odd sine power</title>
                <p>
                  If <m>m=2k+1</m> is odd, write
                  <me>
                    \int \sin^m x\cos^n x\, dx=\int (1-\cos^2x)^k\cos^n x\sin x\, dx
                  </me>
                  and use the substitution <m>u=\cos x, du=-\sin x\, dx</m>.
                </p>
              </li>
              <li>
                <title>Odd cosine power</title>
                <p>
                  If <m>n=2k+1</m> is odd, write
                  <me>
                    \int \sin^m x\cos^n x\, dx=\int \sin^m x(1-\sin^2x)^k\cos x \, dx
                  </me>
                  and use the substitution <m>u=\sin x, du=\cos x\, dx</m>.
                </p>
              </li>
              <li>
                <title>Even powers</title>
                <p>
                  If <m>m</m> and <m>n</m> are both even use <m>\displaystyle\sin^2 x=\frac{1-\cos 2x}{2}</m> and
                  <m>\displaystyle\cos^2 x=\frac{1+\cos 2x}{2}</m> to reduce to a lower power of <m>\cos 2x</m>.
                </p>
              </li>
            </ol>
          </p>
        </statement>
    </algorithm>

    <algorithm xml:id="proc_int_tansec">
        <title>Integrating <m>\tan^m x\sec^n x</m></title>
        <statement>
          <p>
            Let <m>m</m> and <m>n</m> be nonnegative integers.
            When computing
            <me>
              \int \tan^m x\sec^n x \, dx
            </me>
            use the following strategies. 
            <ol>
              <li>
                <title>Odd tangent power</title>
                <p>
                  If <m>m=2k+1</m> is odd and <m>n</m> is positive, write
                  <me>
                    \int \tan^m x\sec^n x \, dx=\int (\sec^2 x-1)^k\sec^{n-1} x\sec x\tan x \, dx
                  </me>
                  and use the substitution <m>u=\sec x, du=\sec x\tan x\, dx</m>.
                </p>
              </li>
              <li>
                <title>Even secant power</title>
                <p>
                  If <m>n=2k</m> is even and positive, write
                  <me>
                    \int \tan^m x\sec^n x \, dx=\int (\tan^2 x+1)^{k-1}\tan^m x\sec^2 x\, dx
                  </me>
                  and use the substitution <m>u=\tan x, du=\sec^2 x\, dx</m>.
                </p>
              </li>
              <li>
                <title>Even tangent power, odd secant power</title>
                <p>
                  If <m>m</m> is even and <m>n</m> is odd,
                  express everything in terms of <m>\sec x</m> and possibly use integration by parts.
                </p>
              </li>
              <li>
                <title>Tangent power</title>
                
                
                <p>
                    If <m>n=0</m>, use the identity <m>\tan^2 x=\sec^2 x-1</m> and strategies from the previous cases. 
                </p>
              </li>
            </ol>
          </p>
        </statement>
    </algorithm>

    <example xml:id="eg_odd_sin_power">
        <title>Odd sine power</title>
        <statement>
            <p>
                Compute <m>\displaystyle \int \sin^3x \cos^2 x\, dx</m>.
            </p>
        </statement>
        <solution>
            <p>
                Peel off a factor of <m>\sin x</m> and use the substitution <m>u=\cos x</m>, <m>du=-\sin x</m>: 
                <md>
                  <mrow> \int \sin^3x \cos^2 x\, dx   \amp = \int \sin^2x \cos^2 x \sin x\, dx </mrow>
                  <mrow> \amp = \int (1-\cos^2x) \cos^2 \sin x\, dx</mrow>
                  <mrow> \amp  = -\int (1-u^2)u^2\, du \amp (u=\cos x, du=-\sin x dx)</mrow>
                  <mrow> \amp = -\frac{1}{3}u^3+\frac{1}{5}u^5+C</mrow>
                  <mrow> \amp = -\frac{1}{3}\cos ^3 x+\frac{1}{5}\cos^5 x+C</mrow>
                </md>
            </p>
        </solution>
    </example>
    <example xml:id="eg_even_powers">
        <title>Even powers</title>
        <statement>
            <p>
                Compute <m>\displaystyle \int \sin^2 x\cos^4 x\, dx</m>.
            </p>
        </statement>
        <solution>
            <p>
               Both powers are even. We use the square identity to reduce powers across the board: 
               <md>
                <mrow> \int \sin^2 x\cos^4 x\, dx \amp = \int \frac{1}{2}(1-\cos 2x)\left(\frac{1}{2}(1+\cos 2x)\right)^2\, dx </mrow>
                <mrow> \amp = \frac{1}{8}\int (1-\cos 2x)(1+\cos 2x)^2\, dx</mrow>
                <mrow> \amp = \frac{1}{8}\int 1+\cos 2x-\cos^2 2x-\cos^3 2x\, dx
                </mrow>
                <mrow> \amp = \frac{1}{8}\int 1-\cos^2 2x+\sin^2 x\cos x\, dx \amp (\cos^3 x=(1-\sin^2 x)\cos x)</mrow>
                <mrow> \amp =\frac{1}{8}\int \frac{1}{2}-\frac{1}{4}\cos 4x+\underset{u^2}{\underbrace{\sin^2 2x}}\, \underset{\frac{du}{2}}{\underbrace{\cos 2x\, dx}} \amp (\cos 2x=\frac{1}{2}(1+\cos 4x))</mrow>
                <mrow> \amp = \frac{1}{16}x-\frac{1}{64}\sin 4x+\frac{1}{48}\sin^3 2x+C \amp (u=\sin 2x, du=2\cos 2x dx)</mrow>
               </md>.
            </p>
        </solution>
    </example>
    <example xml:id="eg_even_sec_power">
        <title>Even secant power</title>
        <statement>
            <p>
                Compute <m>\displaystyle \int \sec^4 x\, dx</m>.
            </p>
        </statement>
        <solution>
            <p>
                Peel off a factor of <m>\sec^2 x</m> and use the substitution <m>u=\tan x</m>, <m>du=\sec^2 x dx</m>:
                <md>
                  <mrow> \int \sec^4 x\, dx\amp = \int (\tan^2 x+1)\, \underset{u}{\underbrace{\sec^2 x\, dx}}</mrow>
                  <mrow> \amp = \frac{1}{3}\tan^3 x+\tan x+C \amp (u=\tan x, du=\sec^2 x\, dx)</mrow>
                </md>.
            </p>
        </solution>
    </example>
    
    <example xml:id="eg_odd_tan_power">
        <title>Odd tangent power</title>
        <statement>
            <p>
                Compute <m>\displaystyle \int \tan^5 x\sec^7 x\, dx</m>.
            </p>
        </statement>
        <solution>
            <p>
                Peel off a factor of <m>\tan x\sec x</m> and use the substitution <m>u=\sec x</m>, <m>du=\sec x\tan x</m>:
                <md>
                  <mrow> \int \tan^5 x\sec^7 x\, dx \amp = \int (\sec^2-1)^2\sec^6 x \, \underset{du}{\underbrace{\sec x\tan x\, dx}}</mrow>
                  <mrow> \amp = \int u^{10}-2u^{8}+u^6\, du \amp (u=\sec x, du=\sec x\tan x dx)</mrow>
                  <mrow> \amp = \frac{1}{11}\sec^{11}x-\frac{2}{9}\sec^9 x+\frac{1}{7}\sec x+C</mrow>
                </md>.
            </p>
        </solution>
    </example>

    <example xml:id="eg_even_tan_odd_sec">
        <title>Even tangent power, odd secant power</title>
        <statement>
            <p>
                Compute  <m>\displaystyle \int \sec^3 x\, dx</m>.
            </p>
        </statement>
        <solution>
            <p>
                Not much we can do here besides integration by parts: 
                <md>
                  <mrow>\int \sec^3 x\, dx \amp = \sec x\tan x-\int \sec x\tan^2 x\, dx \amp (u=\sec x, v'=\sec^2 x)</mrow>
                  <mrow> \amp = \sec x\tan x-int \sec^3 x-\sec x\, dx \amp (\tan^2 x=\sec^2 x-1) </mrow>
                  <mrow> \amp = \sec x\tan x+\ln\abs{\sec x+\tan x}-\int \sec^3 x\, dx</mrow>
                </md>.
                We've shown that 
                <me>
                  \int \sec^3 x\, dx=\sec x\tan x+\ln\abs{\sec x+\tan x}-\int \sec^3 x\, dx
                </me>.
                Doing some algebra and solving for <m>\int \sec^3 x\, dx</m>, we conclude that 

                <me>
                  \int \sec^3 x\, dx=\frac{1}{2}\sec x\tan x+\frac{1}{2}\ln\abs{\sec x+\tan x}+C. 
                </me>.
            </p>
        </solution>
    </example>
    <example xml:id="eg_tan_power">
        <title>Tangent power</title>
        <statement>
            <p>
                Compute  <m>\displaystyle \int \tan^5 x \, dx</m>.
            </p>
        </statement>
        <solution>
            <p>
                Following the suggestion of <xref ref="proc_int_tansec"/> we 
                <me>
                  \tan^5 x=(\tan^2 x)^2\tan x=(\sec^4 x-2\sec^2 x+1)\tan x
                </me>,
                from which we conclude 
                <md>
                  <mrow>\int \tan^5 x\, dx \amp = \int \sec^4 x\tan x-2\sec^2 x\tan x+\tan x\, dx </mrow>
                  <mrow> \amp = \int \underset{u^3}{\underbrace{\sec^3 x}}\, \underset{du}{\underbrace{\sec x\tan x}}-2\underset{u}{\underbrace{\sec x}} \, \underset{du}{\underbrace{\sec x\tan x}}+\tan x\, dx </mrow>
                  <mrow> \amp =\frac{1}{4}\sec^4 x-\sec^2 x-\ln\abs{\cos x}+C</mrow>
                </md>.
                
            </p>
        </solution>
    </example>


</section>